new approach for verse: fuel based semantics

coq/verse/verse.sig
@@ -1,0 +1,24 @@
+Val  : Type
+Exp  : Type
+Op : Type
+nat : Type
+
+opAdd : Op
+opGt  : Op
+opInt : Op
+
+
+Int   : nat -> Val
+Prim  : Op -> Val
+Tuple : Val -> Val
+Lam   : (Val -> Exp) -> Val
+
+Ret   : Val -> Exp
+App   : Val -> Val -> Exp
+Seq   : Exp -> Exp -> Exp
+Unify : Exp -> Exp -> Exp
+Exists : (Val -> Exp) -> Exp
+Or    : Exp -> Exp -> Exp
+Fail  : Exp 
+One   : Exp -> Exp
+All   : Exp -> Exp
