coq/verse/densem.v
@@ -1,0 +1,284 @@
+Require Import Coq.Vectors.Fin.
+Require Coq.Vectors.VectorDef.
+Require List.
+Import List.ListNotations.
+
+Require Export ssreflect.
+Require Export Coq.Classes.RelationClasses.
+Require Import structures.Sets.
+
+(* This file defines a "denotational" semantics for Verse as *sets of values*.
+   This semantics is not correct, but illustrative of difficulties.
+
+   For example, the denotation of the expression "2 || 3" is the set
+   {2,3}. This isn't right (as it loses the order), but using sets makes it
+   easy to define the interpretation of "∃".
+
+   The key idea is that the interpretation of "∃ x. e" is the set of all
+   values in the interpretation of "e", using any value w for x.  We might
+   write that mathematically as:
+
+        { x | x ∈ eval (w :: env) e, for w in W }
+
+   Some points about this file:
+
+    - This semantics uses {} (the emptyset) as the denotation of both FAIL and
+      WRONG
+  
+           what should the semantics of "(true + 1) || 2" be?  should it be
+           WRONG or should it be 2?
+
+    - This semantics also uses {} as the denotation of both FAIL and "bottom".
+
+      The denotation function is threaded with a "fuel" value to deal with non
+      termination.  If there is not enough fuel, then the denotation is
+      bottom.
+
+      The idea is that for any *terminating* expression there should be some
+      amount of "fuel" that is enough to fully define its semantics. However,
+      there is a twist: with a set based semantics, by giving more fuel, we
+      may get a larger set of results. For example,
+
+               " 2 || fact 5"
+
+      will produce the singleton set {2} for small values of fuel and {2, 120}
+      with more fuel.
+
+      This is BAD news for "all". If this term gathers all values in the set
+      into a tuple, how does it know when to stop? Sometimes the denotation of
+
+             all(2 || fact 5)
+
+      is the set {<2>} and sometimes it is the set {<2,120>}. The first set is
+      not a subset of the second, so our denotation is not
+      monotonic. Computations may return different results (not more results)
+      given more fuel.
+
+    - This is less bad news for "one" (but still not good). In this version,
+      we cannot define the semantics for "one" without the axiom of
+      choice. And this would probably not be monotonic because as we generate
+      larger sets, AC may pick out different elements. But if we can get the
+      ordering nailed down, then we may be in better shape.
+
+    - This isn't a good denotational semantics as I'm using closures as the
+      denotations of functions. But equality is syntactic, so there are
+      functions that are extensionally equal that are distinguished by the
+      semantics.  For example, \x. x + 1 would not unify with \x. 1 + x.
+
+*)
+
+
+Set Implicit Arguments.
+
+Inductive Op : Type := op_Add | op_Gt | op_Int.
+
+Inductive Val (n: nat) : Type := 
+  | Var   : Fin.t n -> Val n
+  | Int   : nat -> Val n
+  | Prim  : Op -> Val n
+  | Pair  : Val n -> Val n -> Val n   (* todo: generalize to n-tuples *)
+  | Lam   : Exp (S n) -> Val n
+
+with Exp (n : nat): Type :=
+  | Ret    : Val n -> Exp n
+  | App    : Val n -> Val n -> Exp n  
+  | Seq    : Exp n -> Exp n -> Exp n
+
+  | Unify  : Exp n -> Exp n -> Exp n   
+  | Exists : Exp (S n) -> Exp n
+  | Or     : Exp n -> Exp n -> Exp n 
+  | Fail_  : Exp n
+  | One    : Exp n -> Exp n 
+  | All    : Exp n -> Exp n  
+.
+
+Arguments Int {_}.
+Arguments Prim {_}.
+Arguments Fail_ {_}.
+
+(* This is our domain of values (W): numbers, primitives, pairs of values 
+   and closures *)
+Inductive W : Type := 
+  | IntV   : nat -> W
+  | PrimV  : Op -> W
+  | PairV  : W -> W -> W
+  | LamV   : forall {n}, VectorDef.t W n -> Exp (S n) -> W   (* closure *)
+.
+
+Import SetNotations.
+
+
+Section Monad.
+
+Definition M (A : Type) := P A.  (* set of values of type A *)
+
+Definition WRONG {A} : M A := ∅.
+Definition FAIL {A} : M A := ∅.
+Definition UNIT  {A} : A -> M A := fun x => ⌈ x ⌉.
+Definition UNION {A} : M A -> M A -> M A := Union. 
+Definition INTER {A} : M A -> M A -> M A := Intersection.
+
+Definition SEQ {A} : M A -> M A -> M A := 
+  fun s1 s2 => (fun x => (exists y, s1 y) /\ s2 x).
+
+(* Because there is no order, we need something like the axiom of choice 
+   to pick a distinguished element of the set. And is AC monotonic? I dunno....
+
+*)
+Definition ONE {A} : M A -> M A := 
+  fun s => s.
+
+(* Note: since we only have binary pairs, this is a bit odd. ALL works when
+   there are two values in the set. However, having n-tuples would also
+   produce a non-monotonic operator. As the number of potential results grows,
+   then the size of the tuple *also* grows. This is not ideal.
+*)
+Definition ALL : M W -> M W := 
+  fun s => (fun y => match y with 
+                       | PairV w1 w2 => s w1 /\ s w2
+                       | _ => False
+                       end).
+
+(* Merge togther the result of the function f applied to every w in W *)
+Definition EXISTS {A} (f : A -> M A) : M A := 
+  fun x => exists w, x ∈ f w.
+
+End Monad.
+
+
+Section Semantics.
+
+Definition Env (n : nat) := VectorDef.t W n.
+Definition lookupEnv {n} (e : Env n) (x : Fin.t n) : W := VectorDef.nth e x. 
+
+(* semantics of values *)
+Fixpoint evalVal {n} (env : Env n) (V : Val n) : W :=
+  match V with 
+  | Var v => lookupEnv env v
+  | Lam e => LamV env e
+  | Pair v1 v2 => PairV (evalVal env v1) (evalVal env v2)
+  | Int k => IntV k
+  | Prim o => PrimV o
+  end.
+ 
+Definition evalPrim (o : Op) (w : W) : M W := 
+  match o , w with 
+  (* addition *)
+  | op_Add , PairV (IntV j) (IntV k) => UNIT (IntV (j+k))
+  | op_Add , _ => WRONG
+  (* Gt *)
+  | op_Gt  , PairV (IntV j) (IntV k) => 
+      if Nat.leb k j then UNIT ( IntV j ) else FAIL
+  | op_Gt , _ => WRONG
+  (* type test: identity function on Int, fails when given a non int value *)
+  | op_Int , IntV k => UNIT ( IntV k )
+  | op_Int , _ => FAIL
+  end.
+
+Import VectorDef.VectorNotations.
+
+(* semantics of expressions *)
+
+Fixpoint evalExp (m:nat) {n : nat} (env: Env n) (e: Exp n) : M W :=  
+  match m with 
+  | 0 => FAIL
+  | S m' => match e with 
+           | Ret v => 
+               UNIT (evalVal env v)
+
+           | Fail_ => FAIL
+
+           | Or e1 e2 => UNION (evalExp m' env e1) (evalExp m' env e2)
+
+           | Unify e1 e2 => INTER (evalExp m' env e1) (evalExp m' env e2)
+
+           | Seq e1 e2 => SEQ (evalExp m' env e1) (evalExp m' env e2)
+
+           | App e v => 
+               let w := evalVal env v in
+               match evalVal env e with                      
+                 | (LamV env1 e1) => evalExp m' (VectorDef.cons _ w _ env1) e1
+                 | PrimV p => evalPrim p w
+                 | _ => WRONG   (* non-function application *)
+               end
+
+           | Exists e => 
+               EXISTS (fun w => evalExp m' (VectorDef.cons _ w _ env) e)
+
+           | One e => ONE (evalExp m' env e)
+
+           | All e => ALL (evalExp m' env e)
+           end
+  end.
+
+End Semantics.
+
+
+Import VectorDef.VectorNotations.
+
+(* Examples *)
+
+(* exists x. x = 3 ; x *)
+Definition ex0 : Exp 0 := 
+  Exists (Seq (Unify (Ret (Var F1)) (Ret (Int 3))) (Ret (Var F1))).
+
+Lemma evex0 : exists n, UNIT (IntV 3) ≃ evalExp n (@VectorDef.nil _) ex0.
+exists 4. 
+simpl.
+split.
+- unfold EXISTS.
+  intros x xIn. inversion xIn.
+  exists (IntV 3). 
+  econstructor.
+  exists (IntV 3).
+  repeat econstructor; eauto.
+  repeat econstructor; eauto.
+- unfold EXISTS.
+  intros x xIn. inversion xIn.
+  cbv in H.
+  move: H => [[y h1] h2].  inversion h2. subst.
+  inversion h1. subst. inversion H. subst. inversion H0. subst.
+  auto.
+Qed.
+
+(* exists x. x = 3 | x = 4 *)
+
+Definition ex1 : Exp 0 := 
+ Exists (Or (Unify (Ret (Var F1)) (Ret (Int 3)))
+            (Unify (Ret (Var F1)) (Ret (Int 4)))).
+
+Lemma evex1 : exists n, evalExp n (@VectorDef.nil _) ex1 ≃ (⌈ IntV 3 ⌉ ∪ ⌈IntV 4⌉).
+exists 10.
+simpl.
+unfold EXISTS.
+split.
+- intros x xIn. inversion xIn. clear xIn.
+  inversion H. subst.
+  inversion H0. subst.
+  inversion H1. inversion H2. subst.
+  left. auto.
+  inversion H0. inversion H2. inversion H3. subst.
+  right. auto.
+- intros x xIn. inversion xIn; subst; clear xIn; inversion H; clear H.
+  + exists (IntV 3).
+    constructor. constructor. auto. auto.
+  + exists (IntV 4).
+    right. constructor. auto. auto.
+Qed.
+
+(* 
+    exists x. x 1 = 2 ; x 1 
+*)
+
+Definition ex2 : Exp 0 := 
+  Exists (Seq (Unify (App (Var F1) (Int 1)) (Ret (Int 2)))
+              (App (Var F1) (Int 1))).
+
+(* We can show that "2" is in the meaning of this expression *)
+Lemma evex2 : exists n, IntV 2 ∈ evalExp n (@VectorDef.nil _) ex2.
+Proof.
+  exists 5.
+  exists (LamV (@VectorDef.nil _) (Ret (Int 2))).
+  cbv.
+  split; eauto. exists (IntV 2). constructor; eauto. constructor; eauto.
+Qed.
