coq/verse/densemLabeledResult.v
@@ -1,0 +1,2106 @@
+Require Export ssreflect.
+Require Export Coq.Classes.RelationClasses.
+Require Export Coq.Classes.Morphisms.
+
+Require Coq.Sorting.Sorted.
+Require Coq.Lists.List.
+
+Require structures.Option.
+Require Import structures.Sets.
+Require Import structures.Monad.
+
+(* autosubst2 "generated" syntax *)
+Require Import fintype.
+Require Import verse.syntax.
+
+Set Implicit Arguments.
+
+(* This file defines a "denotational" semantics for Verse.
+
+   W* == (label * result W) -> Prop
+
+   The label records which branch of an "Or" we are in
+   The option records whether that branch diverges or not
+   If a branch fails, that label will not be in the set
+
+   NOTE: In Coq, the type A -> Prop represents a set of "A"s. In 
+   this semantics, we have an invariant that for any l, there is at most *one*
+   x in the set. So really instead of a set of values, we have 
+   a partial mapping of labels to values.
+
+   W* == Set of (label * option W) 
+
+   Can we capture this invariant in the type some how? I'm not sure
+
+     o  W* == label -> option A   
+ 
+        is not the same because it requires a deciable function, not a relation
+
+     o  W* == label -> option W -> Prop 
+
+        doesn't enforce the invariant, because it is just currying the above
+
+     o  W* == { S : P (label * option W) | partial_function S }
+
+        enforces invariant but is annoying to work with
+
+*)
+
+(* --------------------------------------------------------- *)
+(* --------------------------------------------------------- *)
+(* "deriving" Eq for syntax                                  *)
+(* --------------------------------------------------------- *)
+(* --------------------------------------------------------- *)
+
+Module EqSyntax.
+
+Module Op. 
+
+Definition eqb (x y : Op) : bool :=
+  match  x , y with
+  | opAdd , opAdd => true
+  | opGt , opGt => true
+  | opInt , opInt => true
+  | _ , _ => false
+  end.
+
+Lemma eqb_eq : forall x y, 
+  eqb x y = true <-> x = y.
+Proof.
+  intros x y. split; destruct x; destruct y; simpl; done.
+Qed. 
+
+Lemma eqb_neq : forall x y, 
+  eqb x y = false <-> x <> y.
+Proof. 
+  intros x y. split; destruct x; destruct y; simpl; done.
+Qed.
+
+End Op.
+
+Fixpoint fin_eqb {n} := 
+  match n return fin n -> fin n -> bool with 
+  | 0 => fun x y => match x with end
+  | S m => fun x y =>
+      match x , y with 
+      | Some x' , Some y' => fin_eqb x' y'
+      | None , None => true
+      | _ , _ => false
+      end
+  end.
+
+Fixpoint Val_eqb {n} (x y : Val n) : bool := 
+  let fix Vals_eqb {n} (xs ys : list (Val n)) := 
+  match xs , ys with
+  | cons x xs , cons y ys => (Val_eqb x y && Vals_eqb xs ys)%bool
+  | nil , nil => true
+  | _ , _ => false
+  end in
+  match x , y with 
+  | var_Val f1 , var_Val f2 => fin_eqb f1 f2
+  | Int n1 , Int n2 => Nat.eqb n1 n2
+  | Prim o1 , Prim o2 => Op.eqb o1 o2
+  | Tuple vs1 , Tuple vs2 => Vals_eqb vs1 vs2
+  | Lam e1 , Lam e2 => Exp_eqb e1 e2
+  | _ , _ => false
+  end
+with Exp_eqb {n} (x y : Exp n) : bool := 
+  match x, y with 
+  | Ret v1 , Ret v2 => Val_eqb v1 v2
+  | App v1 u1 , App v2 u2 => Val_eqb v1 v2 && Val_eqb u1 u2
+  | Seq e1 e2 , Seq e1' e2' => Exp_eqb e1 e1' && Exp_eqb e2 e2'
+  | Unify v1 e2 , Unify v1' e2' => Val_eqb v1 v1' && Exp_eqb e2 e2'
+  | Exists e1 , Exists e1' => Exp_eqb e1 e1'
+  | Or e1 e2 , Or e1' e2' => Exp_eqb e1 e1' && Exp_eqb e2 e2'
+  | Fail , Fail => true
+  | One e1 , One e1' => Exp_eqb e1 e1'
+  | All e1 , All e1' => Exp_eqb e1 e1'
+  | _ , _ => false
+  end.
+
+
+End EqSyntax.
+Import EqSyntax.
+
+
+(* --------------------------------------------------------- *)
+(* --------------------------------------------------------- *)
+(* Syntactic sugar                                           *)
+(* --------------------------------------------------------- *)
+(* --------------------------------------------------------- *)
+
+Definition var_one {n : nat} : fin (S (S n)) := Some None. 
+Definition var_two {n : nat} : fin (S (S (S n))) := Some (Some None). 
+
+Definition bind1 {n} : Exp n -> Exp (S n) -> Exp n := 
+  fun e1 e2 =>
+    Exists (Seq (Unify (var_Val var_zero) (ren_Exp shift e1)) e2).
+
+Definition bind2 {n} : Exp n -> Exp n -> Exp (S (S n)) -> Exp n := 
+  fun e1 e2 e3 =>
+    Exists (Seq (Unify (var_Val var_zero) (ren_Exp shift e1))
+                (Exists (Seq (Unify (var_Val var_zero) (ren_Exp (shift >> shift) e2))
+                          e3))).
+
+Definition app {n} : Exp n -> Exp n -> Exp n := 
+  fun e1 e2 => bind2 e1 e2 (App (var_Val var_one) (var_Val var_zero)).
+
+
+Module VerseNotations.
+
+Declare Scope verse_syntax.
+Delimit Scope verse_syntax with Exp.
+Open Scope verse_syntax.
+
+Notation x0 := (var_Val var_zero).
+Notation x1 := (var_Val var_one).
+Notation x2 := (var_Val var_two).
+
+Notation "⟨⟩" := (Tuple nil) : verse_syntax.
+
+Infix ";;" := Seq (at level 100, right associativity) : verse_syntax.
+
+Infix "≡" := Unify (at level 100, right associativity) : verse_syntax.
+
+Coercion Ret : Val >-> Exp.
+
+Infix "@" := app (at level 71, left associativity) : verse_syntax.
+
+Definition ifthenelse {n} (e1 e2 e3 : Exp n) : Exp n := 
+  One ( Or ( e1 ;; Lam ( ⟨⟩ ≡ x0 ;; ren_Exp shift e2 ) )
+                 ( Lam ( ⟨⟩ ≡ x0 ;; ren_Exp shift e3 ) )) @ ⟨⟩.
+
+Notation "e1 ?? e2 :: e3" := (ifthenelse e1 e2 e3) (at level 70) : verse_syntax.
+
+End VerseNotations.
+
+
+(* --------------------------------------------------------- *)
+(* --------------------------------------------------------- *)
+(* Length indexed vectors *)
+(* --------------------------------------------------------- *)
+(* --------------------------------------------------------- *)
+
+Module Vector. 
+
+Inductive vec (A:Type) : nat -> Type := 
+  | nil : vec A 0
+  | cons : forall {n}, A -> vec A n -> vec A (S n)
+.
+
+Arguments nil {_}.
+Arguments cons {_}{_}.
+
+Fixpoint nth {A}{n} (v : vec A n) : fin n -> A := 
+  match v in vec _ n return fin n -> A with 
+        | nil => null
+        | cons x xs => fun f => match f with 
+                            | Some g => nth xs g
+                            | None => x
+                            end
+        end.
+
+(* 
+Fixpoint eqb {A} {n} (eqA : A -> A -> bool) := 
+  match n return vec _ n -> vec A n -> bool with 
+  | 0 => fun v1 v2 => true
+  | S m => fun v1 v2 => 
+            match v1 , v2 in vec _ m with 
+            | cons x xs , cons y ys => (eqA x y && eqb eqA xs ys)%bool
+            | nil , nil => true
+            | _ , _ => false
+            end
+  end.
+*)
+
+Declare Scope vec_scope.
+Delimit Scope vec_scope with vec.
+Bind Scope vec_scope with vec.
+
+Open Scope vec_scope.
+
+Module VectorNotation.
+Infix "::" := cons (at level 60, right associativity) : vec_scope.
+Notation "[ ]" := nil (format "[ ]") : vec_scope.
+Notation "[ x ]" := (cons x nil) : vec_scope.
+(*
+Notation "[ x ; y ; .. ; z ]" := (cons x (cons y .. (cons z nil) ..))
+  (format "[ '[' x ; '/' y ; '/' .. ; '/' z ']' ]") : vec_scope.
+*)
+End VectorNotation.
+
+End Vector.
+
+(* --------------------------------------------------------- *)
+(* --------------------------------------------------------- *)
+(*                     Labels                                *)
+(* --------------------------------------------------------- *)
+(* --------------------------------------------------------- *)
+
+Module Label.
+
+Declare Scope label_scope.
+Delimit Scope label_scope with label.
+Open Scope label_scope.
+
+Inductive label : Type := 
+   | Top : label
+   | Br  : label -> label -> label   (* sequenced choices *)
+   | L   : label -> label           (* inside a left choice *)
+   | R   : label -> label           (* inside a right choice *)
+.
+
+Module Label.
+
+  Fixpoint compare (l m : label) : comparison := 
+    match l , m with 
+    | L l0 , L m0 => compare l0 m0
+    | R l0 , R m0 => compare l0 m0 
+    | L _  , R _  => Lt
+    | R _ , L _   => Gt
+
+    | Top , Top => Eq
+
+    | Br l1 l2 , Br l3 l4 => 
+        match compare l1 l3 with
+        | Eq => compare l2 l4
+        | o  => o
+        end
+
+    (* these don't matter, we will only compare comparable things *)
+    | L _ , _  => Lt
+    | _   , L _  => Gt
+    | Top , _ => Lt
+    | _   , Top => Gt
+    | Br _ _ , _ => Lt
+    | _   , Br _ _ => Gt
+   
+    end.
+
+  Fixpoint comparable (l1 l2 : label) : bool :=
+    match l1 , l2 with 
+    | L l0 , L m0 => comparable l0 m0
+    | R l0 , R m0 => comparable l0 m0 
+    | L _  , R _  => true
+    | R _ , L _   => true
+    | Top , Top => true
+    | Br l1 l2 , Br l3 l4 => comparable l1 l3 && comparable l2 l4
+    | _ , _ => false
+    end.
+
+  (* During computation, a partial result will have label "Top". However, 
+     if we give the evaluator more fuel, the expression may make 
+     choices, so the label will grow more structure.
+
+          Top ⊑ L Top
+              ⊑ L (R Top) 
+              ⊑ L (R (Top ⋈ Top))
+              ⊑ L (R (L Top ⋈ Top))
+              ⊑ L (R (L Top ⋈ R Top))
+   *)
+  Fixpoint approx (l1 l2 : label) : bool := 
+    match l1 , l2 with 
+    | Top , _ => true 
+    | L l0 , L l1 => approx l0 l1 
+    | R l0 , R l1 => approx l0 l1 
+    | Br l1 l2 , Br l3 l4 => approx l1 l3 && approx l2 l4            
+    | _ , _ => false
+    end.
+
+  Lemma approx_refl : forall l, approx l l = true.
+  Proof. induction l; eauto. simpl. rewrite IHl1. rewrite IHl2. auto. Qed.
+
+  Lemma approx_trans : forall l2 l1 l3, 
+      approx l1 l2 = true -> approx l2 l3 = true -> approx l1 l3 = true.
+  Proof. induction l2. all: intros l1 l3. 
+         all: destruct l1; destruct l3.
+         all: simpl; intros h1 h2; try done. 
+         all: try (apply andb_prop in h1; move: h1 => [h1 h1']).
+         all: try (apply andb_prop in h2; move: h2 => [h2 h2']).
+         all: try (apply andb_true_intro; split; eauto 3).
+         eauto.
+         eauto.
+  Qed.
+
+  Definition eqb l m : bool := 
+    match compare l m with 
+    | Eq => true
+    | _ => false
+    end.
+
+  Definition ltb l m : bool := 
+    match compare l m with 
+    | Lt => true
+    | _ => false
+    end.
+
+  Fixpoint leb l m : bool := 
+    match compare l m with 
+    | Lt => true
+    | Eq => true
+    | _ => false
+    end.
+
+Lemma compare_refl: forall x, compare x x = Eq.
+Proof. induction x.
+       cbv. done. 
+       simpl. rewrite IHx1. rewrite IHx2. done.
+       simpl; auto.
+       simpl; auto.
+Qed.
+
+
+Lemma compare_eq : forall x y, compare x y = Eq <-> x = y.
+Proof. 
+intros x y.
+split.
+- move: y. 
+  induction x; intros y; destruct y.
+  all: simpl.
+  all: try done.
+  all: try (destruct (compare x1 y1) eqn:c1).
+  all: intro c2.
+  all: try done.
+  all: try rewrite (IHx1 y1); auto. 
+  all: try rewrite (IHx2 y2); auto. 
+  all: try rewrite (IHx y); auto. 
+- move: y. induction x; intros y; destruct y.
+  all: simpl.
+  all: try done.
+  all: try (destruct (compare x1 y1) eqn:c1).
+  all: intro c2.
+  all: try (inversion c2; subst; clear c2).
+  all: try rewrite (IHx1 y1); auto. 
+  all: rewrite IHx1 in c1; auto.
+Qed.
+
+
+Lemma compare_transitive: forall y x z o, 
+    compare x y = o -> compare y z = o -> compare x z = o.
+Proof. 
+  move=> y. induction y; intros x z o h1 h2.
+  all: destruct x; destruct z; simpl in *; subst; auto.
+  all: try solve [inversion h2; auto].
+  destruct (compare y1 z1) eqn: c1;
+  destruct (compare x1 y1) eqn: c2.
+  all: try (rewrite compare_eq in c1; subst).
+  all: try (rewrite compare_eq in c2; subst).
+  all: try (rewrite compare_refl).
+  all: try rewrite c2; auto.
+  all: try rewrite c1; auto.
+  all: try solve [inversion h2].
+  + erewrite IHy1 with (o := Lt); auto.
+  + erewrite IHy1 with (o := Gt); auto.
+Qed.
+
+Lemma ltb_notreflexive: forall x, not (ltb x x = true).
+intros x. unfold ltb. rewrite compare_refl. done.
+Qed.
+
+End Label.
+
+Module LabelNotation.
+Infix "⋈" := Br (at level 70, right associativity) : label_scope.
+Infix "=?" := Label.eqb (at level 70) : label_scope.
+Infix "<=?" := Label.leb (at level 70) : label_scope.
+Infix "<?" := Label.ltb (at level 70) : label_scope.
+End LabelNotation.
+  
+Instance LtStrict : StrictOrder (fun x y : label => (Label.ltb x y) = true).
+constructor.
+- intros l h. eapply Label.ltb_notreflexive; eauto.
+- intros x y z. move: z. 
+  induction y; intros z h1 h2; destruct x; destruct z; 
+    cbn in *; try done.
+  + unfold Label.ltb in *.
+    simpl in *.
+    specialize (IHy1 z1). 
+    specialize (IHy2 z2).
+Admitted.
+
+Lemma leb_antisymmetry k1 k2 : 
+  Label.leb k1 k2 = true -> Label.leb k2 k1 = true -> k1 = k2.
+Proof. 
+  move: k2.
+  induction k1; intros k2; destruct k2.
+  all: simpl.
+  all: try done.
+Admitted.
+
+
+End Label.
+
+Import Label.
+
+
+Section PartialFunctions.
+
+Import SetNotations.
+
+(* --------------------------------------------------------- *)
+(* --------------------------------------------------------- *)
+(*      partial functions as sets of pairs                   *)
+(* --------------------------------------------------------- *)
+(* --------------------------------------------------------- *)
+
+(* A set of pairs is a partial function if there is at most one 
+   mapping for any key in the set. NOTE: this definition uses 
+   syntactic equality for values. That means that for values 
+   with multiple representations (i.e. functions) this definition 
+   is too rigid. 
+*)
+Definition partial_function {K}{V}  (S : P (K * V)) := 
+  forall k v1 v2, (k , v1) ∈ S -> (k , v2) ∈ S -> v1 = v2.
+
+(* This predicate defines when a key is in the domain of 
+   the partial function *)
+Definition in_dom {K}{V} (s : P (K * V)) (k : K) : Prop := 
+  exists v, (k,v) ∈ s.
+
+(* Access the canonical list of elements in a finite mapping *)
+Definition elements {K}{V} (R : K -> K -> Prop) (s : P (K * V)) (l : list (K * V)) : Prop := 
+  let LT := fun '(l1,_) '(l2, _)=> R l1 l2 in
+  (mem l = s) /\                        (* memberships are equal *)
+  @Sorted.LocallySorted _ LT l.        (* the list is sorted by the labels *)
+
+
+(*
+Lemma app_cong {A B} {f g : A -> B} : f = g -> forall x, f x = g x.
+intro h. rewrite h. auto. Qed. 
+*)
+
+Lemma smaller_notpresent {K}{V}{R : K -> K -> Prop}`{StrictOrder _ R} (a : K * V) (w : list (K * V)) :
+  List.Forall (let '(l1, _) := a in fun '(l2, _) => R l1 l2) w ->
+  ~(List.In a w).
+Proof. destruct a. 
+       induction w.
+       intros h1 h2. inversion h2.
+       intros h1 h2. simpl in h2. 
+       inversion h1. subst.
+       destruct h2.
+       + rewrite H0 in H2. destruct H. 
+         unfold Irreflexive, complement, Reflexive in *. 
+         eauto.
+       + apply IHw; eauto.
+Qed.
+
+Lemma elements_functional {K}{V}{R : K -> K -> Prop}
+  `{StrictOrder _ R}{e: P (K * V) }{w1 w2} : 
+  partial_function e -> 
+  elements R e w1 -> elements R e w2 -> w1 = w2.
+Proof.
+  move=> pfe.
+  have TR: Transitive (fun '(l1, _) '(l2, _) => R l1 l2).
+  { intros t. unfold Transitive.
+    intros [l1 _][l2 _][l3 _]. eapply H. }
+  unfold elements in *.
+  repeat rewrite <- Sorted.Sorted_LocallySorted_iff.
+  move=> [m1 S1].
+  move=> [m2 S2]. rewrite <- m1 in m2. 
+  apply Sorted.Sorted_StronglySorted in S1; try apply TR.
+  apply Sorted.Sorted_StronglySorted in S2; try apply TR.
+  remember ((fun '(l1, _) '(l2, _) => R l1 l2) : (K * V) -> (K * V) -> Prop) as Rl.
+  move: S1 w2 m2 S2.
+  induction w1.
+  - intros S1 w2 m2 s2. destruct w2. done.
+Admitted.
+(*    
+    unfold mem in m2. 
+    
+    move: m2 => [m21 _].
+    specialize (m21 p ltac:(left; eauto)).
+    inversion m21.
+  - intros S1 w2 m2 S2. destruct w2. 
+    -- move: m2 => [_ m22].
+       specialize (m22 a ltac:(left; eauto)).
+       inversion m22.
+    -- inversion S1. subst.
+       inversion S2. subst.
+       move: (@smaller_notpresent K V R H a w1 H3) => ni1.
+       move: (@smaller_notpresent K V R H p w2 H5) => ni2.
+       have: (a = p). admit. move => h. subst a.
+       apply Sets.mem_cons_inv in m2.
+       f_equal. eapply IHw1; eauto.
+Admitted. *)
+
+End PartialFunctions.
+
+(* --------------------------------------------------------- *)
+(* --------------------------------------------------------- *)
+(*                     Result                                *)
+(* --------------------------------------------------------- *)
+(* --------------------------------------------------------- *)
+
+(* Note: failure is the absence of a result. We don't want it 
+   to be a specific result, because terms will fail in LOTs 
+   of ways and we don't want to keep track of that. *)
+Inductive Result (A : Type) : Type := 
+  | Bottom : Result A
+  | Wrong  : Result A 
+  | Value  : A -> Result A.
+
+Arguments Bottom {_}.
+Arguments Wrong {_}.
+Arguments Value  {_}.
+
+Module R. 
+
+Definition isWrong {A} (r : Result A) : bool := 
+  match r with | Wrong => true | _ => false end.
+Definition isBottom {A} (r: Result A) : bool := 
+  match r with | Bottom => true | _ => false end.
+Definition isValue {A} (r: Result A) : bool := 
+  match r with | Value _ => true | _ => false end.
+
+Definition strict {A} (r1 r2 : Result A) : Result A  := 
+  match r1 , r2 with
+  | Bottom , _ => Bottom
+  | Wrong , _ => Wrong
+  | Value _ , r2 => r2
+  end.
+
+Definition approx {A} (r1 r2 : Result A) : Prop := 
+  match r1 , r2 with 
+  | Bottom , _ => True
+  | Wrong , Wrong => True
+  | Value w1 , Value w2 => w1 = w2
+  | _ , _ => False
+end.
+
+Definition keep {A} (R : A -> A -> bool) (w1 : A) (r : Result A) : bool := 
+  match r with
+  | Value w2 => R w1 w2
+  | Bottom => true
+  | Wrong => false
+  end.
+
+End R.
+
+
+
+(* --------------------------------------------------------- *)
+(* --------------------------------------------------------- *)
+(*                     Domain of values                      *)
+(* --------------------------------------------------------- *)
+(* --------------------------------------------------------- *)
+
+(* This is our domain of values (W): numbers, primitives, tuples of values 
+   and closures *)
+
+Inductive W : Type := 
+  | IntV    : nat -> W
+  | PrimV   : Op -> W
+  | TupleV  : list W -> W
+  | LamV    : forall {n}, Vector.vec W n -> Exp (S n) -> W   (* a closure *)
+.
+
+#[export] Hint Constructors W.
+
+Module W.
+
+(* syntactic equality for values *)
+Fixpoint eqb (x : W) (y : W) : bool := 
+  let fix eqbs (xs : list W) (ys : list W) : bool :=
+    match xs , ys with 
+    | (x :: xs)%list , (y :: ys)%list => (eqb x y && eqbs xs ys)%bool
+    | nil , nil => true
+    | _ , _ => false
+    end 
+  in match x , y with 
+     | IntV x , IntV y => Nat.eqb x y
+     | PrimV x , PrimV y => Op.eqb x y
+     | TupleV xs , TupleV ys => eqbs xs ys
+     | LamV v1 e1 , LamV v2 e2 => false (* todo *)
+     | _ , _ => false
+     end.
+
+End W.
+
+
+(* --------------------------------------------------------- *)
+(* --------------------------------------------------------- *)
+(*                Semantic operators                         *)
+(* --------------------------------------------------------- *)
+(* --------------------------------------------------------- *)
+
+Section Semantics.
+
+Import LabelNotation.
+Import SetNotations.
+Import MonadNotation.
+Import AlternativeNotation.
+
+Local Open Scope monad_scope.
+
+Definition left {A} : (label * A) -> (label * A) := 
+  fun '(l,w) => (L l, w).
+Definition right {A} : (label * A) -> (label * A) := 
+  fun '(l,w) => (R l, w).
+
+
+Definition M (A : Type) := (label * Result A) -> Prop.  
+
+Definition BOTTOM {A} : P (label * Result A) := ⌈ (Top, Bottom) ⌉.
+
+Definition WRONG {A} : P (label * Result A) := ⌈ (Top, Wrong) ⌉.
+
+Definition FAIL {A} : P (label * Result A) := ∅.
+
+Definition UNIT {A} (x : A) : P (label * Result A) := ⌈ (Top, Value x) ⌉.
+
+(* { (L𝑙,𝑤) | (𝑙,𝑤) ∈ 𝑠1 } ∪ {(R𝑙,𝑤) | (𝑙,𝑤) ∈ 𝑠2 } *)
+Definition UNION {A} (s1 s2 : P (label * Result A)) := 
+  fmap left s1 ∪ fmap right s2.
+
+
+(* 
+If the second expression fails, then the whole expression fails, no matter 
+what the first expression is. 
+If the first expression is fail, loop or error, that is the result of the 
+entire expression.
+If the first expression succeeds, then the result is the second expression.
+
+r ; fail    --> fail
+r ; fail    --> fail
+fail  ; r   --> fail
+loop  ; r   --> loop
+error ; r   --> error
+value ; r   --> r 
+
+ *)
+  (* {(𝑙1 ⋈ 𝑙2,𝑤2) | (𝑙1,𝑤1) ∈ 𝑠1, (𝑙2,𝑤2) ∈ 𝑠2} *)
+Definition SEQ {A} s1 s2 :  P (label * Result A)%type :=
+  '(l1, r1) <- s1 ;;
+  '(l2, r2) <- s2 ;;
+  ⌈ (l1 ⋈ l2, R.strict r1 r2) ⌉
+(* add this to make loop ; fail --> loop *)
+    ∪
+  (fun '(l1, r1) => match (l1, r1) with 
+                | (l ⋈ Top, Bottom) => (l, Bottom) ∈ s1
+                | _ => False
+                end).
+
+(* Find the result associated with the *smallest* entry in the set. *)
+Definition ONE {A} (s : P (label * Result A)) : (label * Result A) -> Prop := 
+  fun '(l,w) => 
+    match l , w with 
+    | Top , w => exists k, ((k,w) ∈ s) 
+                /\ (forall k' w', (k', w') ∈ s -> (k <=? k' = true))
+    | _ , _ => False
+    end.
+
+(* Merge togther the result of the function f applied to every w in W.
+
+   - Ensure that we only have one nonfailing result per label. If a label has
+     a different mapping (for any picked value), then do not include it in the
+     set. (TODO: make it WRONG instead?)  *)
+                                          
+Definition EXISTS {A} (f : A -> M A) : M A := 
+  fun '(l,r) => (exists w, (l,r1) ∈ f w) 
+           /\ ((forall w' r2, (l, r2) ∈ f w' -> (r1 = r2 -> r = r1))      (* all agree *)
+            \/ (exists w' r2, (l, r2) ∈ f w' -> (r1 <> r2 /\ r = WRONG)))  (* some discrepancy *)
+              (* make ∃x.x fail *)
+.
+
+
+(* Could value w1 be represented by the entry? *)
+Definition keep (w1 : W) (entry : label * Result W) : bool := 
+  match entry with
+  | (l, Some w2) => W.eqb w1 w2
+  | (l, None) => true
+  end.
+(*  Intersection fails if its argument fails
+    and diverges if its argument diverges *)
+  (* { (l2, 𝑤2) | (𝑙2,𝑤2) ∈ 𝑠2, 𝑤1 = 𝑤2} *)
+Definition INTER (w : W) : M W -> M W := Sets.filter (keep w).
+
+
+(* The 'elements' proposition asserts that a set s is finite and contains the ordered 
+   list of entries (i.e. labeled results). *)
+Definition ALL : M W -> M W := 
+  fun s => fun '(l,r) => 
+    match l , r with 
+    | Top , Some (TupleV ws) => 
+        exists entries , elements (fun x y => x <? y = true) s entries 
+               /\ (List.map snd entries = List.map Some ws) 
+                                          (* all of the results must succeed *)
+    | Top , None => exists l, (l , None) ∈ s    (* if any of the results diverge, ALL diverges *)
+    | _   , _ => False                         (* if there are no results, ALL fails *)
+    end.
+
+
+
+End Semantics.
+
+(* --------------------------------------------------------- *)
+(* --------------------------------------------------------- *)
+(*                Evaluator                                  *)
+(* --------------------------------------------------------- *)
+(* --------------------------------------------------------- *)
+
+Section Eval.
+
+Open Scope vec_scope.
+Import Vector.VectorNotation.
+
+
+Definition Env (n : nat) := Vector.vec W n.
+Definition lookupEnv {n} (e : Env n) (x : fin n) : W := Vector.nth e x. 
+
+(* semantics of values *)
+Fixpoint evalVal {n} (env : Env n) (V : Val n) : W :=
+  let evalVals (vs : list (Val n)) : list W := List.map (evalVal env) vs in
+  match V with 
+  | var_Val v => lookupEnv env v
+  | Lam e => LamV env e
+  | Tuple vs => TupleV (evalVals vs)
+  | Int k => IntV k
+  | Prim o => PrimV o
+  end.
+
+Definition evalVals {n} (env : Env n) := (List.map (evalVal env)).
+
+Definition evalPrim (o : Op) (w : W) : M W := 
+  match o , w with 
+  (* addition *)
+  | opAdd , TupleV (cons (IntV j) (cons (IntV k) nil)) => UNIT (IntV (j+k))
+  | opAdd , _ => WRONG
+  (* Gt *)
+  | opGt  , TupleV (cons (IntV j) (cons (IntV k) nil)) =>
+      if Nat.leb k j then UNIT ( IntV j ) else FAIL
+  | opGt , _ => WRONG
+  (* type test: identity function on Int, fails when given a non int value *)
+  | opInt , IntV k => UNIT ( IntV k )
+  | opInt , _ => FAIL
+  end.
+
+(* semantics of expressions *)
+
+Fixpoint evalExp (m:nat) {n : nat} (e: Exp n) : Env n -> M W :=  
+  match m with 
+  | 0 => fun env => BOTTOM
+  | S m' => match e with 
+           | Ret v => fun env => UNIT (evalVal env v)
+
+           | Fail => fun env => FAIL
+
+           | Or e1 e2 => fun env => UNION (evalExp m' e1 env) (evalExp m' e2 env)
+
+           | Unify v1 e2 => fun env => INTER (evalVal env v1) (evalExp m' e2 env)
+
+           | Seq e1 e2 => fun env => SEQ (evalExp m' e1 env) (evalExp m' e2 env)
+
+           | App e v => fun env =>
+               let w := evalVal env v in
+               match evalVal env e with                      
+                 | LamV env1 e1 => evalExp m' e1 (w :: env1)
+                 | PrimV p => evalPrim p w
+                 | _ => WRONG   (* non-function application *)
+               end
+
+           | Exists e => fun env => EXISTS (fun w => evalExp m' e (w :: env))
+
+           | One e => fun env => ONE (evalExp m' e env)
+
+           | All e => fun env => ALL (evalExp m' e env)
+           end
+  end.
+
+Lemma eval_Ret {m' n} {v} : evalExp (S m') (Ret v) = fun (env : Env n) => UNIT (evalVal env v).
+Proof. reflexivity. Qed.
+Lemma eval_Or  {m' n} {e1 e2} : 
+   evalExp (S m') (Or e1 e2) = fun (env : Env n) => UNION (evalExp m' e1 env) (evalExp m' e2 env).
+Proof. reflexivity. Qed.
+Lemma eval_App  {m' n} {e v} : 
+   evalExp (S m') (App e v) = fun (env : Env n) => let w := evalVal env v in
+               match evalVal env e with                      
+                 | LamV env1 e1 => evalExp m' e1 (w :: env1) 
+                 | PrimV p => evalPrim p w
+                 | _ => WRONG   (* non-function application *)
+               end.
+Proof. reflexivity. Qed.
+Lemma eval_Seq {m' n} {e1 e2} : 
+  evalExp (S m') (Seq e1 e2) = fun (env : Env n) => SEQ (evalExp m' e1 env) (evalExp m' e2 env).
+Proof. reflexivity. Qed.
+Lemma eval_Unify {m' n} {v1 e2} : 
+  evalExp (S m') (Unify v1 e2) = fun (env : Env n) => INTER (evalVal env v1) (evalExp m' e2 env).
+Proof. reflexivity. Qed.
+Lemma eval_Exists {m' n} {e} : 
+  evalExp (S m') (Exists e) = fun (env : Env n) => EXISTS (fun w => evalExp m' e (Vector.cons w env)).
+Proof. reflexivity. Qed.
+Lemma eval_One {m' n} {e} : 
+  evalExp (S m') (One e) = fun (env : Env n) => ONE (evalExp m' e env).
+Proof. reflexivity. Qed.
+Lemma eval_All {m' n} {e} : 
+  evalExp (S m') (All e) = fun (env : Env n) => ALL (evalExp m' e env).
+Proof. reflexivity. Qed.
+
+End Eval.
+
+Create HintDb evalExp.
+Hint Rewrite @eval_Ret @eval_Or @eval_App @eval_Seq @eval_Unify @eval_Exists @eval_One @eval_All : evalExp.
+
+
+(* --------------------------------------------------------- *)
+(* --------------------------------------------------------- *)
+(* Validity                                                  *)
+(* --------------------------------------------------------- *)
+(* --------------------------------------------------------- *)
+
+
+Section Validity.
+
+Import SetNotations.
+
+(* We want to ensure that all interpretations are "valid". In other words, 
+   the sets are all partial functions. *)
+
+Definition Valid {A} : M A -> Prop := partial_function.
+
+Lemma partial_function_BOTTOM {A} : partial_function (@BOTTOM A).
+  intros k v1 v2 in1 in2. inversion in1. inversion in2. done.
+Qed.
+
+Lemma partial_function_UNIT {A} (x:A) : partial_function (UNIT x).
+  intros k v1 v2 in1 in2. inversion in1. inversion in2. done.
+Qed.
+
+Lemma partial_function_FAIL {A} : partial_function (@FAIL A).
+  intros k v1 v2 in1 in2. inversion in1. 
+Qed.
+
+Lemma partial_function_WRONG {A} : partial_function (@WRONG A).
+  intros k v1 v2 in1 in2. inversion in1. 
+Qed.
+
+Lemma partial_function_UNION {A} (s1 s2 : M A) : partial_function s1 -> partial_function s2 -> partial_function (UNION s1 s2).
+intros pf1 pf2 k v1 v2 in1 in2.
+unfold UNION in *. unfold partial_function in *.
+inversion in1 as [? h1|? h1]; inversion in2 as [? h2|? h2]; subst; clear in1 in2.
+cbv in h1,h2.
+all: move: h1 => [[l1 r1] [h1 h1']]; inversion h1'; subst; clear h1'.
+all: move: h2 => [[l2 r2] [h2 h2']]; inversion h2'; subst; clear h2'.
+eauto.
+eauto.
+Qed.
+
+Lemma partial_function_INTER  
+  (v : W)(s2 : M W) : partial_function s2 -> partial_function (INTER v s2).
+Proof.
+  intros pf k v1 v2 in1 in2.
+  unfold INTER in *. unfold partial_function in *.
+  unfold filter in *.
+  move: in1 => [k1 in1].
+  move: in2 => [k2 in2].
+  eauto.
+Qed.
+
+Lemma partial_function_SEQ {A} (s1 s2 : M A) : partial_function s1 -> partial_function s2 -> partial_function (SEQ s1 s2).
+Proof.
+  move=> pf1 pf2 k v1 v2 in1 in2.
+  unfold partial_function in *.
+  cbn in in1.
+  move: in1 => [[l1 r1] [h1 [[l1' r1'] [h1' h]]]]. inversion h. subst. clear h.
+  move: in2 => [[l2 r2] [h2 [[l2' r2'] [h2' h]]]]. inversion h. subst. clear h.
+  move: (pf1 _ _ _ h1 h2) => E1.
+  move: (pf2 _ _ _ h1' h2') => E2.
+  subst.
+  auto.
+Qed.
+
+(* The IH doesn't help here because it only talks about individual 
+   sets f w. But we need to reason about all f w. *)
+Lemma partial_function_EXISTS {A} (f : A -> M A) : 
+  (forall w, partial_function (f w)) -> partial_function (EXISTS f).
+Proof.
+intros ih k v1 v2 in1 in2.
+move: in1 => [[w1 in1] p1].
+move: in2 => [[w2 in2] p2].
+eapply p1; eauto.    
+Qed.
+
+Lemma partial_function_ONE (e : M W) : partial_function e -> partial_function (ONE e).
+Proof.
+  intros pf k v1 v2 in1 in2.
+  unfold ONE, partial_function in *.
+  destruct k; try done.
+  move: in1 => [k1 [h1 h1']].
+  move: in2 => [k2 [h2 h2']].
+  have LE1: (Label.leb k1 k2 = true); eauto.
+  have LE2: (Label.leb k2 k1 = true); eauto.
+  move: (Label.leb_antisymmetry _ _ LE1 LE2) => eq. subst.
+  eauto.
+Qed.
+
+Lemma map_Some_inv {A} {l l0 : list A} : list_map Some l = list_map Some l0 -> l = l0.
+Proof. move: l0. 
+       induction l; intros [|l0] h; inversion h; subst; f_equal.
+       eapply IHl; eauto.
+Qed.
+
+Lemma partial_function_ALL (e : M W) : partial_function e -> partial_function (ALL e).
+Proof.
+  intros pfe k v1 v2 in1 in2.
+  destruct k; try done.
+  destruct v1; try done.
+  destruct v2; try done.
+  destruct w; try done.
+  destruct w0; try done.
+  move: in1 => [w1 [in1 p1]].
+  move: in2 => [w2 [in2 p2]].
+  - f_equal. f_equal.
+    have EQ : (w1 = w2). eapply elements_functional; eauto. subst.
+    rewrite p1 in p2.
+    apply map_Some_inv in p2. auto.
+  - destruct w; try done. 
+    destruct in1 as [xs [h1 h2]].
+    destruct in2 as [l' h3].
+    move: h1 => [h1 SS]. subst.
+    apply mem_In in h3.
+    apply List.in_map with (f := snd) in h3. rewrite h2 in h3. simpl in h3.
+    rewrite List.in_map_iff in h3.
+    move: h3 => [? [h3 _]]. done.
+  - destruct v2. destruct w; try done.
+    destruct in1 as [l' h3].
+    destruct in2 as [xs [h1 h2]].
+    move: h1 => [h1 SS]. subst.
+    apply mem_In in h3.
+    apply List.in_map with (f := snd) in h3. rewrite h2 in h3. simpl in h3.
+    rewrite List.in_map_iff in h3.
+    move: h3 => [? [h3 _]]. done.
+    auto.
+Qed.
+
+Lemma partial_function_evalPrim {o w} :
+   partial_function (evalPrim o w).
+Proof.
+  destruct o; destruct w; simpl.
+  all: try eapply partial_function_WRONG.
+  all: try eapply partial_function_UNIT.
+  all: try destruct l.
+  all: try destruct w.
+  all: try destruct l.
+  all: try destruct w.
+  all: try destruct l.
+  all: try eapply partial_function_WRONG.
+  all: try eapply partial_function_UNIT.
+  destruct (Nat.leb n0 n).
+  all: try eapply partial_function_UNIT.
+  all: try eapply partial_function_FAIL.
+Qed.
+
+Lemma partial_function_evalExp : forall k n (env : Env n) e , partial_function (evalExp k e env).
+intros k. induction k.
+- intros. cbn. eapply partial_function_BOTTOM.
+- intros.
+  destruct e.
+  + simpl. eapply partial_function_UNIT.
+  + repeat rewrite eval_App.    
+    remember (evalVal env v0) as w. cbv zeta.
+    destruct (evalVal env v).
+    all: try eapply partial_function_WRONG.
+    eapply partial_function_evalPrim.
+    eapply IHk.
+  + repeat rewrite eval_Seq. eapply partial_function_SEQ; eauto.
+  + repeat rewrite eval_Unify. eapply partial_function_INTER; eauto.
+  + repeat rewrite eval_Exists.
+    eapply partial_function_EXISTS. intro w; eauto.
+  + repeat rewrite eval_Or.
+    eapply partial_function_UNION; eauto.
+  + simpl.
+    eapply partial_function_FAIL; eauto.
+  + rewrite eval_One.
+    eapply partial_function_ONE; eauto.
+  + rewrite eval_All.
+    eapply partial_function_ALL; eauto.
+Qed.
+
+End Validity.
+
+
+
+(* --------------------------------------------------------- *)
+(* --------------------------------------------------------- *)
+(* Monotonicity                                              *)
+(* --------------------------------------------------------- *)
+(* --------------------------------------------------------- *)
+
+
+Section Monotonicity.
+
+Import SetNotations.
+Import MonadNotation.
+
+(* one interpretation approximates another when
+
+   for each entry in s1: 
+      1. if it has succeeded, 
+          a. it continues to succeed in s2 with the same label
+      2. if it has bottomed, 
+          a. it could stay bottom, with a potentially bigger label
+          b. it could succeed, with a potentially bigger label
+          c. it could fail and won't be in s2
+          (( this condition is trivial ))
+      3. if it fails (i.e. is not in the first set)
+          - it should continue to fail and all bigger labels shouldn't be in s2
+         we can express this using the contrapositive:
+            everything in s2 should be approximated by something in s1
+         
+
+We need (1) to know that successful values do not change with more fuel.
+We need (3) for the case of ONE
+  We need to know that there are no new "smaller" elements when we add more fuel.
+
+
+ *)
+
+
+Definition entry_approx {A}(e1 e2 : label * Result A) : Prop := 
+  match e1 , e2 with 
+  | (l1 , Some v1), (l2, Some v2) => Label.approx l1 l2 = true /\ v1 = v2
+  | (l1 , None), (l2 , _) => Label.approx l1 l2 = true
+  | _ , _ => False
+  end.
+
+Lemma entry_approx_label {A:Type} {l1 r1 l2 r2}: 
+  entry_approx (A:=A) (l1, r1) (l2, r2) -> Label.approx l1 l2 = true.
+destruct r1; destruct r2; simpl; eauto.
+tauto.
+Qed.
+
+Definition approx {A} (s1 s2 : M A) : Prop := 
+  (forall l1 v, (l1, Some v) ∈ s1 -> ((l1, Some v) ∈ s2)) /\
+  (forall e2, e2 ∈ s2 -> exists e1, (e1 ∈ s1) /\ entry_approx e1 e2).
+
+
+(*
+  (forall l1,   ((l1, None) ∈ s1 -> exists l2, ((exists v, (l2, Some v) ∈ s2) \/ (l2, None) ∈ s2)
+                                    /\ Label.approx l1 l2 = true)) /\  (* 2bc *)
+  (forall l2 v, (l2 , Some v) ∈ s2 -> (exists l1, ((l1 ,Some v) ∈ s1) /\ Label.approx l1 l2 = true) \/  (* 1a *)
+                                 exists l1, ((l1, None) ∈ s1)   /\ Label.approx l1 l2 = true) /\  (* 2c *)
+  (forall l2, (l2 , None) ∈ s2 -> exists l1, Label.approx l1 l2 = true /\ ((l1, None) ∈ s1)).          (* 2b *)
+*)
+
+(*
+Definition approx {A} (s1 s2 : M A) : Prop := 
+  (forall l1 v, ((l1, Some v) ∈ s1 -> exists l2, ((l2, Some v) ∈ s2) /\ Label.approx l1 l2 = true)) /\  (* 1a *)
+  (forall l1,   ((l1, None) ∈ s1 -> exists l2, ((exists v, (l2, Some v) ∈ s2) \/ (l2, None) ∈ s2)
+                                    /\ Label.approx l1 l2 = true)) /\  (* 2bc *)
+  (forall l2 v, (l2 , Some v) ∈ s2 -> (exists l1, ((l1 ,Some v) ∈ s1) /\ Label.approx l1 l2 = true) \/  (* 1a *)
+                                 exists l1, ((l1, None) ∈ s1)   /\ Label.approx l1 l2 = true) /\  (* 2c *)
+  (forall l2, (l2 , None) ∈ s2 -> exists l1, Label.approx l1 l2 = true /\ ((l1, None) ∈ s1)).          (* 2b *)
+*)
+
+Lemma approx_refl {A} : forall (s : M A), approx s s.
+Proof. intros s. unfold approx. repeat split. 
+       eauto using Label.approx_refl. 
+       intros e2 In2.
+       exists e2. split; auto. destruct e2. destruct o; simpl;        eauto using Label.approx_refl.        
+Qed.
+Lemma approx_trans {A} : forall (s1 s2 s3 : M A), approx s1 s2 -> approx s2 s3 -> approx s1 s3.
+Proof. 
+Admitted.
+(*
+intros s1 s2 s3 [a11 [a12 a13]] [a21 [a22 a23]]. 
+       repeat split. 
+       - intros l1 v inV. admit.
+       - intros l v inV. 
+Admitted. 
+         destruct (a22 l v inV) as [|[l2 [h3 h4]]].
+         destruct (a12 l v H) as [|[l1 [h1 h2]]]. 
+         left; auto.
+         right. exists l1. split; auto.
+         right.
+         destruct (a13 l2 h4) as [l1 [h5 h6]].
+         exists l1. split. eapply Label.approx_trans; eauto. auto.
+       - intros l3 l3N.
+         destruct (a23 l3 l3N) as [l2 [h1 l2N]].
+         destruct (a13 l2 l2N) as [l1 [h2 l1N]].
+         exists l1. split. eapply Label.approx_trans; eauto. auto.
+Qed. *)
+
+
+Ltac rewrite_approx := 
+  match goal with 
+  [ H2 : Label.approx ?l2 ?l2' = true |- _ ] => rewrite -> H2 ; clear H2
+  end.
+
+
+Lemma SEQ_monotone {A} {s1 s2 s1' s2' : M A} : 
+  approx s1 s1' -> approx s2 s2' -> approx (SEQ s1 s2) (SEQ s1' s2').
+Proof.
+  intros [A1 A1'] [A2 A2'].
+  unfold SEQ. unfold approx in *.
+  split.
+  + intros l v h.
+    move: h => [[l0 v0] [h1 h2]].
+    move: h2 => [[l1 v1] [h2 h3]].
+    destruct v0 as [v0|].
+  - simpl in h3. inversion h3. subst. clear h3.
+    move: (A1 _ _ h1) => h1'.
+    move: (A2 _ _ h2) => h2'.
+    eexists. split; eauto.
+    eexists. split; eauto.
+    econstructor; eauto.
+  - simpl in h3. inversion h3.
+  + intros e h.
+    move: h => [[l0' v0'] [h1 h2]].
+    move: h2 => [[l1' v1'] [h2 h3]].
+    inversion h3. subst. clear h3.
+    move: (A1' _ h1) => [e1' [h1' h1'']].
+    move: (A2' _ h2) => [e2' [h2' h2'']].
+    destruct e1' as [l0 v0]. 
+    destruct e2' as [l1 v1].
+    destruct v1. destruct v1'.
+    all: destruct v0. 
+    all: destruct v0'; try done.
+    all: simpl in h1''; try done.
+    destruct h2''. subst.
+    destruct h1''. subst.
+    ++ eexists. split. 
+       eexists. split; eauto. simpl.
+       eexists. split; eauto. simpl.
+       eauto.
+       simpl. rewrite H0. rewrite H. auto.
+    ++ destruct h2''. subst. 
+      eexists. split.
+       eexists. split; eauto.
+       eexists. split; eauto. simpl. auto.
+       simpl. rewrite h1''. 
+       rewrite H. auto.
+    ++ destruct h2''. subst. eexists. split.
+       eexists. split; eauto. simpl.
+       eexists. split; eauto. simpl. eauto.
+       simpl. rewrite h1''. rewrite H. auto.
+    ++ simpl in h2''. subst. destruct h1''. subst.
+       eexists. split.
+       eexists. split; eauto. simpl.
+       eexists. split; eauto. simpl.
+       eauto.
+       simpl. rewrite H. rewrite h2''. auto.
+    ++ simpl in h2''.       
+       eexists. split.
+       eexists. split; eauto. simpl.
+       eexists. split; eauto. simpl.
+       eauto.
+       simpl. rewrite h1''. rewrite h2''. auto.
+    ++ simpl in h2''.
+       eexists. split.
+       eexists. split; eauto. simpl.
+       eexists. split; eauto. simpl.
+       eauto.
+       simpl. rewrite h1''. rewrite h2''. auto.
+Qed.
+
+(*
+  repeat split.
+  - (* some s => some s' *)
+    intros l v lIn.
+    destruct l; cbv in lIn; try done. 
+    move: lIn => [w1 ?]. go. 
+    unfold approx in *. go. 
+    specialize (H3 _ _ H2). move: H3 => [l2' h2].
+    specialize (H4 _ _ H1). move: H4 => [l1' h1]. clear H0 H5 H7 H.
+    go.
+    exists (l1' ⋈ l2'). split.
+    eexists.
+    repeat split; eauto.
+    simpl. rewrite H0. rewrite H4. auto.
+  - (* some s' => some s \/ none *)
+    intros l2 v lIn. 
+    destruct l2; try done. cbn in lIn.
+    move: lIn => [x lIn]. go.
+    unfold approx in *. go.
+    destruct (H0 _ _ H2) as [h2|h2];
+    destruct (H _ _ H1) as [h1|h1].
+    all: move: h1 => [l1' h1]; move: h2 => [l2' h2]; go.
+    + left. cbn.
+      exists (l1' ⋈ l2').
+      repeat split.
+      eexists. split; eauto.
+      rewrite H8. rewrite H10. done.
+    + right.
+      exists (l1' ⋈ l2'). 
+      cbn.
+      repeat split. 
+      right.
+      eexists. repeat split; eauto.
+      rewrite H8. rewrite H10. done.
+    + right.
+      exists (l1' ⋈ l2').  
+      cbn.
+      repeat split.  
+      left.
+      eexists. repeat split; eauto.
+      simpl. rewrite H8. rewrite H10. done.
+    + right.
+      exists (l1' ⋈ l2').  
+      cbn.
+      repeat split. 
+      right.
+      eexists. repeat split; eauto.
+      rewrite H8. rewrite H10. done.
+  - intros l2 l2I. 
+    destruct l2; try done.
+    cbn in l2I.
+    destruct l2I as [h2|h2].
+    all: try (move: h2 => [w2 h2]; go).
+    all: unfold approx in *; go.
+    all: try (destruct w2).
+    all: try (destruct (H7 _ H1) as [l1' h7]).
+    all: try (destruct (H _ _ H1) as [h1|h1]).
+    all: try (move: h1 => [l1' h1]).
+    all: try (destruct (H5 _ H2) as [l2' h5]).
+    all: try (destruct (H0 _ _ H2) as [h2|h2]).
+    all: try (move: h2 => [l2' h2]).
+    all: go.
+    all: exists (l1' ⋈ l2'); repeat split; simpl; cbn.
+    all: try rewrite H6; try rewrite H10; try reflexivity.
+    all: try rewrite H8; try rewrite H9; try reflexivity.
+    all: try solve [left; eauto].
+    all: try solve [right; eauto].
+Qed. *)
+
+(*
+Ltac ind1 l1' h2 := 
+    match goal with 
+      | [ H1 : (?l1 , Some ?v) ∈ ?s1 ,
+          H2 : forall l v, (l, Some v) ∈ ?s1 -> _ |- _ ] => 
+          move: (H2 _ _ H1) => [l1' h1] ; clear H2
+    end.
+*)
+
+
+Lemma ONE_monotone {s2 s2' : M W} : 
+  approx s2 s2' -> approx (ONE s2) (ONE s2').
+Proof.
+  intros [A1 A2].
+  unfold ONE , approx in *.
+  split.
+  - intros l1 v1 h. destruct l1; try done. 
+    move: h => [k [h1 h2]].
+    move: (A1 _ _ h1) => h3.
+    exists k. split; eauto.
+    intros k' w' In'. 
+    move: (A2 _ In') => [[k0 v0] [h4 h5]].
+    move: (h2 _ _ h4).
+    move: (entry_approx_label h5).
+    clear.
+    move: k0 k'.
+    induction k.
+    all: move=> k0 k' h1 h2.
+    all: destruct k0 eqn:E0; simpl in h2; try done.
+    all: destruct k' eqn:E'; simpl in h1; try done.
+    all: simpl.
+Abort.
+(*  - intros [l2 v2][h2 h3].
+    move: (A2 _ h3) => [[l1 v1] [h1 A3]].
+    exists (l1, v1). split; eauto.
+    split; auto.
+    destruct v1; destruct v2; simpl in *; auto.
+    move:A3 => [h4 ->]. auto.
+Qed.
+*)
+
+      
+Lemma INTER_monotone {w}{s2 s2' : M W} : 
+  approx s2 s2' -> approx (INTER w s2) (INTER w s2').
+Proof.
+  intros [A1 A2].
+  unfold INTER , approx, filter, In in *. 
+  split.
+  - intros l1 v1 h.
+    move: h => [h1 h2].
+    split. eauto. eauto.
+  - intros [l2 v2][h2 h3].
+    move: (A2 _ h3) => [[l1 v1] [h1 A3]].
+    exists (l1, v1). split; eauto.
+    split; auto.
+    destruct v1; destruct v2; simpl in *; auto.
+    move:A3 => [h4 ->]. auto.
+Qed.
+
+(*
+  repeat split.
+  all: intros.
+  + destruct l1; cbn in *; try done.
+    go. 
+    ind1 l1' h1.
+    match goal with 
+      | [ H1 : (?l1 , Some ?v) ∈ s2 ,
+          H2 : forall l v, (l, Some v) ∈ s2 -> _ |- _ ] => 
+          move: (H2 _ _ H1) => [l2' h2] ; clear H2
+    end.
+    exists (l1' ⋈ l2').
+    go.
+    repeat split; eauto.
+    simpl.
+    rewrite_approx.
+    rewrite_approx.
+    reflexivity.
+  + (* some s' => some s \/ none *)
+    destruct l2; cbn in *; try done.
+    go.
+    match goal with 
+      | [ H1 : (?l1 , Some ?v) ∈ s1' ,
+          H2 : forall l v, (l, Some v) ∈ s1' -> _ |- _ ] => 
+          specialize (H2 _ _ H1); destruct H2 as [[l1' h1]|h1] end.
+    match goal with 
+      | [ H1 : (?l1 , Some ?v) ∈ s2' ,
+          H2 : forall l v, (l, Some v) ∈ s2' -> _ |- _ ] => 
+          specialize (H2 _ _ H1); destruct H2 as [[l2' h2]|h2] end.
+    all: go.
+    ++ left. 
+       exists (l1' ⋈ l2'). 
+       repeat split; eauto.
+       rewrite_approx.
+       rewrite_approx.
+       auto.
+    ++ 
+      match goal with 
+      | [ H1 : (?l1 , Some ?v) ∈ s2' ,
+          H2 : forall l v, (l, Some v) ∈ s2' -> _ |- _ ] => 
+          specialize (H2 _ _ H1) end.
+
+Qed. *)
+
+Lemma EXISTS_monotone {A} {f f' : A -> M A} :
+  (forall w, approx (f w) (f' w)) ->
+  approx (EXISTS f) (EXISTS f').
+Proof.
+  intros hA.
+  unfold EXISTS, approx in *.
+  split.
+  - intros l v h0.
+    move: h0 => [[w h0] h1].
+    move: (hA w) => [hA1 hA2].
+    split.
+    exists w. eauto.
+    intros w' r' wIn'.
+    
+
+    eapply h1. 
+Admitted.
+
+
+Lemma evalExp_monotone : forall k n (env : Env n) e , approx (evalExp k e env) (evalExp (S k) e env).
+intros k. induction k.
+- intros. admit. 
+- intros.
+  destruct e.
+  + simpl. eapply approx_refl.
+  + repeat rewrite eval_App.    
+    remember (evalVal env v0) as w. cbv zeta.
+    destruct (evalVal env v).
+    all: try eapply approx_refl.
+    eapply IHk.
+  + repeat rewrite eval_Seq. eapply SEQ_monotone; eauto.
+  + repeat rewrite eval_Unify. eapply INTER_monotone; eauto.
+  + repeat rewrite eval_Exists.
+    eapply EXISTS_monotone. intro w; eauto.
+  + repeat rewrite eval_Or.
+Admitted.
+
+End Monotonicity.
+
+(* --------------------------------------------------------- *)
+(* --------------------------------------------------------- *)
+(* Finite semantics                                          *)
+(* --------------------------------------------------------- *)
+(* --------------------------------------------------------- *)
+
+Require Import Logic.PropExtensionality.
+
+Section FiniteSemantics.
+
+Import SetNotations.
+Import List.ListNotations.
+Import MonadNotation.
+Import LabelNotation.
+
+Open Scope list_scope.
+Open Scope monad_scope.
+
+Lemma singleton_mem {A}{x:A} : ⌈ x ⌉ = mem ([ x ]%list).
+Proof. 
+  eapply Extensionality_Ensembles.
+  rewrite mem_singleton_eq.
+  reflexivity.
+Qed.
+
+Lemma fmap_mem {A B}{f : A -> B}{s} :
+  mem (List.map f s) = fmap f (mem s).
+Proof. 
+Admitted.
+
+Lemma filter_mem {A}{f : A -> bool}{s} :
+  mem (List.filter f s) = filter f (mem s).
+Proof. 
+Admitted.
+
+Lemma bind_cong {A B}{m1 m2 : P A}{k1 k2 : A -> P B} : 
+  (m1 = m2) -> (forall x, k1 x = k2 x) -> bind m1 k1 = bind m2 k2.
+Proof. 
+  intros -> R.
+  cbv.
+  eapply Extensionality_Ensembles.
+  split; intros x [a [h1 h2]].
+    rewrite -> R in h2; exists a; eauto.
+    rewrite <- R in h2; exists a; eauto.
+Qed.
+
+Lemma bind_mem {A B} (m : list A) (k : A -> list B) : 
+  mem (bind m k) = bind (mem m) (fun y => mem (k y)).
+Proof. 
+  induction m.
+  - eapply Extensionality_Ensembles.
+    cbv. split.
+    intros x xIn. done.
+    intros x [y [z w]]. done.
+  - cbn.
+    rewrite union_mem.
+    rewrite IHm.
+    eapply Extensionality_Ensembles.
+    split.
+    + intros x xIn. inversion xIn; subst; clear xIn.
+    ++ exists a. split. left; auto. auto.
+    ++ move: H => [a' [aIn xIn]].
+       exists a'. split. right. auto. auto.
+    + intros x [a' [[h1|h1] h2]]. 
+      ++ subst. econstructor; eauto.
+      ++ right. exists a'. split; eauto.
+Qed.
+
+Lemma UNIT_mem {A} : forall (x : A), 
+    UNIT x = mem ([(Top, Some x)]).
+Proof.
+  intro x. unfold UNIT. eapply singleton_mem.
+Qed.
+
+Lemma UNION_mem {A}{l1 l2: list (label * Result A)} : 
+  UNION (mem l1) (mem l2) = mem (List.map left l1 ++ List.map right l2).
+Proof.
+  unfold UNION.
+  rewrite union_mem.
+  repeat rewrite fmap_mem.
+  reflexivity.
+Qed.
+
+
+Lemma INTER_mem {x:W}{xs:list (label * Result W)} : 
+  INTER x (mem xs) = mem (List.filter (keep x) xs).
+Proof. 
+  unfold INTER.
+  rewrite filter_mem.
+  reflexivity.
+Qed.
+
+
+Lemma SEQ_mem {A}{l1 l2: list (label * Result A)} :
+  SEQ (mem l1) (mem l2) = 
+    mem ( '(l1, r1) <- l1 ;;
+          '(l2, r2) <- l2 ;;
+          [ (l1 ⋈ l2, strictly r1 r2) ] ).
+Proof.
+  unfold SEQ.
+  rewrite -> bind_mem.
+  apply bind_cong.
+  reflexivity.
+  intros [l0 r0].
+  rewrite -> bind_mem.
+  apply bind_cong.
+  reflexivity.
+  intros [k0 r1].
+  rewrite singleton_mem.
+  reflexivity.
+Qed.
+
+
+Definition union_map {A B} (m : list A) (k : A -> P B) : P B :=
+  List.fold_left Union (List.map k m) Empty_set.
+
+Lemma SEQ_mem' {A}{l1: list (label * Result A)}{s2} :
+  SEQ (mem l1) s2 = 
+    union_map l1 (fun '(l1 , r1) => 
+          '(l2, r2) <- s2 ;;
+          ⌈ (l1 ⋈ l2, strictly r1 r2) ⌉).
+Proof.
+  unfold SEQ.
+  induction l1.
+  - cbv.
+    eapply Extensionality_Ensembles.
+    split. intros x [y [h xIn]]. done. intros x xIn. done.
+  - 
+Admitted.
+
+End FiniteSemantics.
+
+Create HintDb mem.
+Hint Rewrite @UNIT_mem @UNION_mem @INTER_mem @SEQ_mem : mem.
+
+
+(* --------------------------------------------------------- *)
+(* --------------------------------------------------------- *)
+(* Examples                                                  *)
+(* --------------------------------------------------------- *)
+(* --------------------------------------------------------- *)
+
+Section Examples.
+
+Import SetNotations.
+Import VerseNotations.
+Import Vector.VectorNotation.
+Import LabelNotation.
+
+Ltac process := 
+  repeat match goal with 
+  | [H : True |- _ ] => clear H
+  | [H : ?a ∈ ⌈ ?a ⌉ |- _ ] => clear H
+  | [H : ?a ∈ ⌈ ?b ⌉ |- _ ] => inversion H; clear H; subst
+  | [H : ?A /\ ?B |- _ ] => inversion H; clear H; subst
+  | [H : ?x ∈ UNIT ?a |- _ ] => inversion H; clear H; subst
+  | [H : UNIT ?a ?x |- _ ] => inversion H; clear H; subst
+  | [H : Some ?a = Some ?b |- _ ] => inversion H; clear H; subst
+  | [H : ⌈ ?a ⌉ ?b |- _ ] => inversion H; clear H; subst
+  | [ |- forall x , _ ] => intros ? 
+  | [H : (exists h, _ ) |- _ ] => move: H => [? H]
+  | [ H : match ?x with _ => _ end |- _ ] => 
+      (destruct x; try done; auto; let n:=numgoals in guard n <= 1) + idtac "too many goals"
+  end.
+
+Ltac go := process;auto.
+
+Hint Unfold UNIT ONE EXISTS.
+Hint Constructors Ensembles.Singleton.
+
+(*
+Lemma f_equal_mem {A}{l1 l2 : list A}: l1 = l2 -> mem l1 ≃ mem l2.
+Admitted. *)
+Lemma P_In {A}{f : P A}{x} : (f x) -> x ∈ f. cbv. auto. Qed.
+
+
+(* 3 = 3 || 4 = 4 || 5 = 5 *)
+Definition exb : Exp 0 := Or (Int 3 ≡ Int 3) (Or (Int 4 ≡ Int 4) (Int 5 ≡ Int 5)).
+
+Example exb_example : evalExp 10 exb Vector.nil = 
+  mem ((L Top, Some (IntV 3)) :: (R (L Top), Some (IntV 4)) :: (R (R Top),Some (IntV 5)) :: nil).
+unfold exb. autorewrite with evalExp.
+unfold evalVal.
+autorewrite with mem.
+f_equal.
+Qed.
+
+Lemma In_extensionality {A} {s1 s2 : P A} : 
+  (forall x, (x ∈ s1) <-> x ∈ s2) -> s1 = s2.
+Proof.
+  intros h.
+  eapply Extensionality_Ensembles.
+  split. intros x xIn; eapply h; eauto.
+  intros x xIn; eapply h; eauto.
+Qed.
+
+Lemma In_mem : forall (A : Type) (x : A) (l : list A), x ∈ mem l <-> List.In x l.
+Admitted.
+
+(* ∃ x. x = (1 || 2) ;; x *)
+Definition ex_two : Exp 0 := bind1 (Or (Int 1) (Int 2)) x0.
+
+Lemma W_eqb_eq (w1 w2: W) : W.eqb w1 w2 = true <-> w1 = w2.
+Admitted.
+
+Lemma ev_ex_two1 : evalExp 10 ex_two Vector.nil =
+                     mem ((L Top ⋈ Top, Some (IntV 1)) :: (R Top ⋈ Top, Some (IntV 2)) :: nil).
+Proof.
+unfold ex_two,bind1. asimpl.
+autorewrite with evalExp.
+unfold evalVal, lookupEnv, Vector.nth, var_zero.
+eapply In_extensionality.
+intros [l r].
+rewrite In_mem.
+repeat rewrite UNIT_mem.
+rewrite UNION_mem.
+Opaque INTER SEQ mem. cbn.
+Transparent INTER SEQ mem.
+split.
++ move=>[[w wIn] _].
+  cbn in wIn.
+  move: wIn => [[l0 r0][ h1 [[l1 r1] [h2 h3]]]].
+  inversion h3; subst; clear h3.
+  unfold UNIT in h2. inversion h2; subst; clear h2.
+  have C: ((w = IntV 1 /\ l0 = L Top) \/ (w = IntV 2 /\ l0 = R Top)).
+  { unfold INTER in h1.
+    rewrite <- filter_mem in h1.
+    rewrite In_mem in h1.
+    cbn in h1.
+    destruct (W.eqb w (IntV 1)) eqn:E1.
+    rewrite W_eqb_eq in E1. subst. cbn in h1. inversion h1; try done. inversion H. subst.
+    left. split; auto.
+    destruct (W.eqb w (IntV 2)) eqn:E2.
+    rewrite W_eqb_eq in E2. subst. inversion h1; try done. inversion H. subst.
+    right. auto.
+    destruct h1.
+  }
+  rewrite INTER_mem in h1.
+  rewrite In_mem in h1.
+  destruct C as [[-> ->]|[-> ->]].
+  ++ cbn in h1. inversion h1; try done. inversion H. subst.
+     simpl. left; eauto.
+  ++ cbn in h1. inversion h1; try done. clear h1. inversion H. subst.
+     simpl. right; left; eauto.
++ move=> [h1|[h1|]]; try done; inversion h1; clear h1; subst.
+  split.
+  ++ exists (IntV 1). exists (L Top, Some (IntV 1)). cbv. split; eauto. econstructor.
+Admitted.
+(*
+     exists (Top, Some (IntV 1)). split; try econstructor; eauto.
+  ++ intros w' r' h.
+     have C : (r' = Some (IntV 1)).
+     { cbn in h.
+       move: h => [[l0 r0] [h1 h2]].
+       move: h2 => [[l1 r1] [h2 h3]].
+       inversion h3; subst; clear h3.
+       inversion h2; subst; clear h2.
+       rewrite INTER_mem in h1.
+       rewrite In_mem in h1.
+       cbn in h1.
+       destruct (W.eqb w' (IntV 1)) eqn:E1. 
+       rewrite W_eqb_eq in E1. subst. 
+       destruct h1. inversion H. done.
+       simpl in H. done.
+       destruct (W.eqb w' (IntV 2)) eqn:E2.
+       rewrite W_eqb_eq in E2. subst. 
+       destruct h1; inversion H. inversion h1.
+     } subst.  auto.
+  ++ admit.
+Admitted. *)
+
+Lemma INTER_two : forall w l1 v1 l2 v2 s, 
+  INTER w (mem ((L l1, Some v1) :: (R l2, Some v2) :: nil)) = s -> 
+  ((w = v1 /\ s = mem ((L l1, Some v1) :: nil)) \/
+   (w = v2 /\ s = mem ((R l2, Some v2) :: nil))).
+Proof.
+Admitted.
+
+       (* prove that there is only one y 
+       rewrite INTER_mem in h.
+       rewrite UNIT_mem in h.
+       simpl in h.
+       destruct (W.eqb w' (IntV 3)) eqn:E1.
+       rewrite W_eqb_eq in E1. subst. simpl in h.
+       rewrite SEQ_mem in h. simpl in h. inversion h. inversion H. auto.
+       inversion H.
+       destruct (W.eqb w' (IntV 4)) eqn:E2. 
+       rewrite W_eqb_eq in E2. subst.
+       rewrite SEQ_mem in h. simpl in h. inversion h. inversion H. auto.
+       rewrite SEQ_mem in h. simpl in h. inversion h.  *)
+
+
+(* ∃ x. x = (1 || 2) ;; exists y. y = (3 || 4) ;; < x , y > *)
+Definition ex_four : Exp 0 := 
+  bind2 (Or (Int 1) (Int 2)) (Or (Int 3) (Int 4)) (Tuple (cons x1 (cons x0 nil))).
+
+Lemma ev_ex_four1 : (L Top ⋈ (L Top ⋈ Top), 
+                      Some (TupleV (cons (IntV 1) (cons (IntV 3) nil))))
+                      ∈ evalExp 30 ex_four Vector.nil.
+Proof.
+  unfold ex_four, bind2.
+  autorewrite with evalExp. 
+  asimpl.
+  autorewrite with evalExp.
+  simpl.
+  unfold lookupEnv, Vector.nth, var_zero, var_one.
+  autorewrite with mem. simpl.
+  split.
+  - exists (IntV 1). 
+    autorewrite with mem. simpl.
+    exists (L Top, Some (IntV 1)). split; eauto.
+    simpl.
+    exists (L Top ⋈ Top, Some (TupleV (IntV 1 :: IntV 3 :: nil))). 
+    split. 2: econstructor; eauto.
+    split.
+    -- cbn.
+       exists (IntV 3). 
+       exists (L Top, Some (IntV 3)). 
+       rewrite INTER_mem. rewrite In_mem.
+       simpl. split; eauto.
+       exists (Top,  Some (TupleV (IntV 1 :: IntV 3 :: nil))). 
+       split. econstructor; eauto.
+       econstructor; eauto.
+    -- intros w' r' h.
+       move: (@INTER_two w' Top (IntV 3) Top (IntV 4) _ ltac:(reflexivity)) => [[h0 h1]| [h0 h1]].
+       subst. rewrite h1 in h. clear h1.
+       rewrite UNIT_mem in h. rewrite SEQ_mem in h. rewrite In_mem in h. simpl in h.
+       inversion h; try done. inversion H. done.
+       subst. rewrite h1 in h. clear h1.
+       autorewrite with mem in h. simpl in h.
+       inversion h; try done. 
+
+  - intros w' r' h.
+    move: (@INTER_two w' Top (IntV 1) Top (IntV 2) _ ltac:(reflexivity)) => [[h0 h1]| [h0 h1]];
+    rewrite h1 in h; clear h1; subst w'.
+    unfold SEQ in h. simpl in h.
+Admitted.
+
+
+
+
+
+Eval cbv in evalExp 10 Vector.nil ex_four.
+
+Lemma label_comparable_SEQ {A}{s1 s2 : M A}{ l1 l2 } :
+  label_comparable s1 l1 -> label_comparable s2 l2 ->
+  label_comparable (SEQ s1 s2) (l1 ⋈ l2).
+Proof.
+  unfold label_comparable.
+  move=> h1 h2.
+  move=> k [v h3]. unfold SEQ in h3.
+  destruct k; try done.
+  simpl.
+  rewrite (h1 k1).
+  2: 
+  rewrite (h2 k2).
+  3: 
+    destruct v; reflexivity.
+  destruct v; cbn in h3.
+  go. econstructor; eauto.
+  destruct h3. go. econstructor; eauto.
+  go. econstructor; eauto.
+  destruct v; cbn in h3.
+  go. econstructor; eauto.
+  destruct h3. go. econstructor; eauto.
+  go. econstructor; eauto.
+Qed.
+
+
+  
+End Example1.
+
+
+
+Module Monotonicity.
+
+
+
+
+Definition contains (w : W) (m : M W ) : Prop := 
+  exists l , (l, Some w) ∈ m.
+
+
+
+(* Examples *)
+
+
+
+(* exists x. x = 3 ; x *)
+Definition ex0 : Exp 0 := 
+  Exists (Seq (Unify (Ret (var_Val var_zero)) (Ret (Int 3))) (Ret (var_Val var_zero))).
+
+Lemma evex0 : exists n, UNIT (IntV 3) ≃ ONE (evalExp n Vector.nil ex0).
+exists 4. 
+cbn. unfold ONE, EXISTS, UNIT.
+split.
+- intros x xIn. go.  
+  exists ((Top ⋈ Top) ⋈ Top)%label.
+  repeat split.
+  -- exists (IntV 3). eexists; repeat econstructor; eauto.
+  -- cbn. go.
+  -- (* label_comparable *)
+    unfold label_comparable, in_dom. go. 
+    cbn in H. go.
+  -- go. cbn in H. go.
+- intros x xIn.
+  cbn in xIn.
+  destruct x; try done.
+  destruct l; try done.
+  cbn in xIn.
+  go.
+Qed.
+
+(* exists x. x = 3 | x = 4 *)
+
+Lemma mem_nil_contra {A}(s : P A): (mem nil ≃ s) -> forall x, (x ∈ s) -> False.
+Proof. intros. unfold mem in H. move: H => [h1 h2].
+specialize (h2 x H0). inversion h2.
+Qed.
+
+Definition ex1 : Exp 0 := 
+ Exists (Or (Unify (Ret (var_Val var_zero)) (Ret (Int 3)))
+            (Unify (Ret (var_Val var_zero)) (Ret (Int 4)))).
+
+Lemma evex1 : exists n, ALL (evalExp n Vector.nil ex1) ≃ UNIT (TupleV (cons (IntV 3) (cons (IntV 4) nil))).
+exists 10.
+unfold ALL, EXISTS.
+split.
+- intros x xIn.
+  destruct x as [l sw].
+  destruct l; try done. 
+  destruct sw as [x|]; cbn in xIn.
+  -- destruct x; try done.
+     move: xIn => [xs ?]. go.
+     have EQ: (l = (IntV 3 :: IntV 4 :: nil)%list).
+     { unfold elements in H. 
+       go.
+       have h1: (List.In (L (Top ⋈ Top), Some (IntV 3)) xs). admit.
+       have h2: (List.In (R (Top ⋈ Top), Some (IntV 4)) xs). admit.
+       admit.
+(*       destruct xs as [|x1 xs].
+       + move: (mem_nil_contra H1 (L (Top ⋈ Top), Some (IntV 3))) => h1. 
+         exfalso. apply h1.
+         cbn.
+         repeat split. eexists. repeat split.
+         go. inversion H4. done.
+         intros. unfold label_comparable. intros k.
+         go. unfold in_dom in H. go. cbn in H. destruct k; try done.
+         destruct k; try done. go. inversion H3. inversion H4. subst. done.
+       + destruct xs as [|x2 xs].
+         *)
+     } subst l.
+     unfold UNIT. econstructor; eauto.
+  -- move: xIn => [l h].
+     go. 
+     destruct l; try done; go. 
+
+- intros x xIn.
+  go.
+  cbn.
+  exists ( (L (Top ⋈ Top), Some (IntV 3)) :: (R (Top ⋈ Top), Some (IntV 4)) :: nil )%list.
+  repeat split.
+  ++ intros x xIn. cbn in xIn. destruct xIn; try done; subst.
+     +++ cbn. repeat split.
+         eexists. repeat split. intros. go. 
+         intros. unfold label_comparable. intros.
+         unfold in_dom in H. go. cbn in H. destruct k; try done.
+         destruct k; try done. go. 
+     +++ destruct H; try done; subst.
+         cbn. repeat split.
+         eexists. repeat split. intros. go. 
+         intros. unfold label_comparable. intros.
+         unfold in_dom in H. go. cbn in H. destruct k; try done.
+         destruct k; try done. go. 
+  ++ intros x xIn. unfold EXISTS in xIn. destruct x. cbn in xIn. go.
+     destruct l; try done. destruct l; try done. go.
+     destruct l; try done. go.
+  ++ repeat econstructor; eauto.
+Admitted.
+
+(* 
+    exists x. x 1 = 2 ; x 1 
+*)
+
+Definition ex2 : Exp 0 := 
+  Exists (Seq (Unify (App (var_Val var_zero) (Int 1)) (Ret (Int 2)))
+              (App (var_Val var_zero) (Int 1))).
+
+(* We can show that "2" is in the meaning of this expression *)
+Lemma evex2 : exists n, exists l, (l, Some (IntV 2)) ∈ evalExp n Vector.nil ex2.
+Proof.
+  exists 20.
+  eexists. unfold ex2. 
+  rewrite -> eval_Exists.
+  unfold EXISTS.
+  remember (LamV Vector.nil (Ret (Int 2))) as w'.
+  remember ((App (var_Val var_zero) (Int 1) ≡ Int 2); App (var_Val var_zero) (Int 1)) as ebody.
+  have VE: forall w', Valid (evalExp 19 (Vector.cons w' Vector.nil) ebody). admit.
+  have EE: (((Top ⋈ Top) ⋈ Top), Some (IntV 2)) ∈ (evalExp 19 (Vector.cons w' Vector.nil) ebody).
+  { subst ebody. subst w'. cbn. eexists. repeat split. }
+  repeat split.
+  - eexists. eauto.
+  - (* need to prove that there is only one possible result *)
+    intros w'' v'.
+    rewrite eval_Seq. unfold SEQ.
+    intro h.
+    destruct h as [w1 [h1 [h2 h3]]].
+    rewrite eval_Unify in h1.
+    unfold INTER in h1.
+    destruct h1 as [h4 h5].
+    cbn in h5. inversion h5. subst.
+    (* here we should know that 
+       - evalExp 17 env e ⊆ evalExp 18 env e 
+       - evalExp 18 env e is Valid, so a partial function
+       - thus v' = Some (IntV 2)
+     *)
+    admit.
+  - (* need to prove that all result labels are compareable with the one that we have. *)
+    
+    intros w'.
+    unfold label_comparable.
+    intro k.
+    intros x.
+    -- unfold WRONG in H. done.
+    -- destruct o; cbn in H1; unfold WRONG in H1; try  done.
+       go.
+    -- unfold WRONG in H. done.
+    -- 
+
+  split; eauto. exists (IntV 2). constructor; eauto. constructor; eauto.
+Qed.
+
+(* 
+What is the meaning of this term?
+if (x=1) then (2 || 3) else 4; x=(1 || 2); if (x=1) then 5 else (6 || 7) 
+
+exists x. if (x=1) then (2 || 3) else 4    ==   [2;3] ∪ [4]
+
+exists x. if (x=1) then (2 || 3) else 4 ; if (x = 1) then 5 else (6 || 7)  
+
+            == [5;5] ∪ [6;7]
+
+               
+
+*) 
+
+
+
+(* 
+
+(* 
+∃x. (if x = 1 then 11 || 22 else 33); x = (1 || 2); (if x= 1 then 44 else 55 || 66)
+
+           < x is 1 >               < x is 2 >
+    == ([11, 22] ; <> ; [44])  ∪ ( [33] ; <> ; [66] ) 
+
+    == 44 ∪ 66
+*)
+
+
+
+
+
+Section ProperInstances.
+
+Import SetNotations.
+Import MonadNotation.
+
+(* --------------------------------------------------------- *)
+(* --------------------------------------------------------- *)
+(* Proper instances for semantic operators                   *)
+(* --------------------------------------------------------- *)
+(* --------------------------------------------------------- *)
+
+
+#[export] Instance UNION_Included_Proper {A} :
+  Morphisms.Proper (Included ==> Included ==> Included) (@UNION A).
+intros s1 t1 R1 s2 t2 R2.
+unfold UNION. 
+eapply union_left. 
++ eapply (@fmap_Included _ _ left) in R1.
+rewrite -> R1.
+eapply sub_union_left.
++ eapply (@fmap_Included _ _ right) in R2.
+rewrite -> R2.
+eapply sub_union_right.
+Qed.
+
+#[export] Instance UNION_Same_set_Proper {A} : Morphisms.Proper (Same_set ==> Same_set ==> Same_set) (@UNION A).
+intros s1 t1 [R1 S1] s2 t2 [R2 S2].
+split; eapply UNION_Included_Proper; eauto.
+Qed.
+
+
+#[export] Instance INTER_Included_Proper : Morphisms.Proper (Logic.eq ==> Included ==> Included) INTER.
+intros s1 t1 -> s2 t2 R2.
+unfold INTER. 
+intros [l w] xIn.
+destruct w; cbn in xIn; try done.
+Admitted.
+
+#[export] Instance INTER_Same_set_Proper : Morphisms.Proper (Logic.eq ==> Same_set ==> Same_set) INTER.
+intros s1 t1 eq s2 t2 [R2 S2]. subst.
+split; eapply INTER_Included_Proper; eauto.
+Qed.
+
+#[export] Instance SEQ_Included_Proper {A} : Morphisms.Proper (Included ==> Included ==> Included) (@SEQ A).
+intros s1 t1 R1 s2 t2 R2.
+unfold SEQ. 
+apply bind_Included_Proper; auto.
+intros [l1 r1].
+apply bind_Included_Proper; auto.
+intros [l2 r2].
+reflexivity.
+Qed.
+
+#[export] Instance SEQ_Same_set_Proper {A} : Morphisms.Proper (Same_set ==> Same_set ==> Same_set) (@SEQ A).
+intros s1 t1 [R1 S1] s2 t2 [R2 S2].
+split; eapply SEQ_Included_Proper; eauto.
+Qed.
+
+(* NOTE: ONE is not monotonic. A larger set gives a different answer. *)
+#[export] Instance ONE_Included_Proper {A} : Morphisms.Proper (Same_set ==> Included) (@ONE A).
+intros s1 t1 [R1 S1].
+unfold ONE. 
+intros [l w] xIn.
+destruct l; cbn in xIn; try done.
+move: xIn => [l [h1 h2]].
+cbn. exists l. split. eapply R1. auto.
+intros k' w' h. apply S1 in h. eauto.
+Qed.
+
+#[export] Instance ONE_Same_set_Proper {A} : Morphisms.Proper (Same_set ==> Same_set) (@ONE A).
+intros s1 t1 R1.
+split; eapply ONE_Included_Proper; eauto. symmetry. auto.
+Qed.
+
+#[export] Instance EXISTS_Included_Proper {A} : Morphisms.Proper ((fun f1 f2 => (forall x, Same_set (f1 x) (f2 x))) ==> Included) (@EXISTS A).
+intros s1 t1 R.
+unfold EXISTS.
+intros [l r] xIn.
+cbn in xIn. cbn.
+move: xIn => [[w h] k].
+move: (R w) => [R1 R2].
+split.
+apply R1 in h. eauto.
+intros w' r' h1.
+move: (R w') => [R1' R2'].
+apply R2' in h1. eauto.
+Qed.
+
+#[export] Instance EXISTS_Same_set_Proper {A} : Morphisms.Proper ((fun f1 f2 => (forall x, Same_set (f1 x) (f2 x))) ==> Same_set) (@EXISTS A).
+intros s1 t1 R1.
+split; eapply EXISTS_Included_Proper; eauto. symmetry. auto.
+Qed.
+
+#[export] Instance ALL_Included_Proper : Morphisms.Proper (Same_set ==> Included) ALL.
+intros s1 t1 R.
+unfold ALL.
+intros [l r] xIn.
+cbn in xIn. destruct l; try done. cbn.
+destruct r. destruct w; try done.
+Admitted.
+
+#[export] Instance ALL_Same_set_Proper : Morphisms.Proper (Same_set ==> Same_set) ALL.
+intros s1 t1 R.  Admitted.
+
+
+
+(*
+Definition InUpTo {A}(eqv : A -> A -> Prop) (s : A -> Prop) (w:A)  : Prop := 
+  exists w', eqv w w' /\ s w'.
+Definition IncludedUpTo {A}(eqv : A -> A -> Prop) (s1 s2 : A -> Prop) : Prop := 
+  (forall x, InUpTo eqv s1 x -> InUpTo eqv s2 x).
+Definition EqUpTo {A} (eqv : A -> A -> Prop) (s1 s2 : A -> Prop) : Prop := 
+  IncludedUpTo eqv s1 s2 /\ IncludedUpTo eqv s2 s1.
+*)
+  
+(*
+Definition EqOption {A} (eqv : A -> A -> Prop) : option A -> option A -> Prop := 
+  fun o1 o2 =>
+    match o1 , o2 with 
+    | None , None => True
+    | Some a1 , Some a2 => eqv a1 a2 
+    | _ , _ => False
+    end.
+Definition EqPair {A}{B} (eqa : A -> A -> Prop) (eqb : B -> B -> Prop) : A * B -> A * B -> Prop := 
+  fun '(a1,y1) '(a2,y2) => eqa a1 a2 /\ eqb y1 y2.
+*)
+
+(*
+Inductive EqV : W -> W -> Prop := 
+  | EqV_IntV : forall k, EqV (IntV k) (IntV k)
+  | EqV_LamV : forall m1 (env1 : Env m1) e1 m2 (env2 : Env m2) e2,
+      (forall w, exists n, 
+          EqUpTo (EqPair (fun l1 l2 => Label.eqb l1 l2 = true) (EqOption EqV)) 
+            (evalExp n (Vector.cons w env1) e1) (evalExp n (Vector.cons w env2) e2)) ->
+      EqV (LamV env1 e1) (LamV env2 e2).
+*)
+
+End ProperInstances.
