coq/verse/densem_iterate.v
@@ -1,0 +1,359 @@
+Require Import Coq.Vectors.Fin.
+Require Coq.Vectors.VectorDef.
+Require List.
+Import List.ListNotations.
+
+Require Export ssreflect.
+Require Export Coq.Classes.RelationClasses.
+
+(* This file defines a denotational semantics for Verse as sets of values. 
+   This semantics is not correct, but illustrative of the difficulties. 
+
+   The interpretation of any expression is as a set of values. For example, 
+   the denotation of " 2 || 3 " is the set {2,3}. This isn't right (as it 
+   loses the order) but it is simple.
+
+   The key idea of this semantics is the interpretation of "∃ x. e" 
+   In this case, we iterate over all potential values and union them together.
+
+   This semantics iterates over all values in the domain, and then 
+
+*)
+
+
+(* Tricky examples:
+
+ How do type errors with || ?
+
+     (true + 1) | 2  ---> 2  
+
+   note: if "exists" iterates over all values, then we will naturally get some failures
+   in 
+
+      exists x. (x + 1 = 2 ; x | x = 3 ; x )
+
+   one possible x could be "true" which would cause the first alternative to 
+   type error. But we don't want to include that type error in the final result.
+
+ How does divergence interact with || ?
+
+     <<diverge>> | 2 ---> ???
+
+ *)
+
+
+Require Import structures.Sets.
+Import SetNotations.
+
+Definition unions {A} : list (P A) -> P A := 
+  List.fold_right Union Empty_set.
+
+Lemma unions_In {A} : 
+  forall (k : P A) (ks: list (P A)), List.In k ks -> k ⊆ unions ks.
+Proof.
+  intros k ks.
+  induction ks. intros h; simpl in h. done.
+  intros h. simpl in h. 
+  intros b bIn. simpl.
+  destruct h. subst. left. auto.
+  right. apply IHks; auto.
+Qed.
+
+Lemma unions_app {A} : forall (l1 l2 : list (P A)),
+    unions (l1 ++ l2) ≃ (unions l1 ∪ unions l2).
+Proof.
+  induction l1. intros l1. simpl. admit.
+  intros l2. simpl. rewrite IHl1. admit.
+Admitted.
+
+Lemma unions_enum_mono {A} : forall (f : A -> P A) l1 l2,  
+  unions (List.map f l1) ⊆ unions (List.map f (l1 ++ l2)).
+Proof.
+  intros f l1 l2.
+  rewrite List.map_app. rewrite unions_app.
+  eauto.
+Qed.
+
+
+(* This version is trying to approximate the semantics given in the verse-densym draft 
+   as closely as possible. *)
+
+
+(* The idea of the "logical" semantics is to provide a sound interpretation of 
+   "lenient" evaluation.
+
+   Then, there would be no need to delay unification steps. They would either succeed or 
+   fail.
+
+   This corresponds to an interpretation of a verse program as a nondeterministic set of 
+   results.
+
+   To be careful about the order of evaluation, we'll do this in the context of 
+   fine-grained CBV language 
+   
+*)
+
+Set Implicit Arguments.
+
+Inductive Op : Type := op_Add | op_Gt | op_Int.
+
+Inductive Val (n: nat) : Type := 
+  | Var   : Fin.t n -> Val n
+  | Int   : nat -> Val n
+  | Prim  : Op -> Val n
+  | Pair  : Val n -> Val n -> Val n   (* todo: generalize to n-tuples *)
+  | Lam   : Exp (S n) -> Val n
+
+with Exp (n : nat): Type :=
+  | Ret    : Val n -> Exp n
+  | App    : Val n -> Val n -> Exp n  (* NOTE ok to make fun an exp *)
+  | Seq    : Exp n -> Exp n -> Exp n
+
+  | Unify  : Exp n -> Exp n -> Exp n   
+  | Exists : Exp (S n) -> Exp n
+  | Or    : Exp n -> Exp n -> Exp n 
+  | Fail_ : Exp n
+  | One   : Exp n -> Exp n 
+  | All   : Exp n -> Exp n 
+  
+.
+
+Arguments Int {_}.
+Arguments Prim {_}.
+Arguments Fail_ {_}.
+
+Section Syntax.
+
+Definition Op_eqb := 
+  fun o1 o2 => match o1 , o2 with 
+            | op_Add , op_Add => true
+            | op_Gt  , op_Gt  => true 
+            | op_Int , op_Int => true
+            | _ , _ => false
+            end.
+
+Definition Op_enum : list Op := [ op_Add ; op_Gt ; op_Int ].
+
+End Syntax.
+
+Section W.
+
+Inductive W : Type := 
+  | IntV   : nat -> W
+  | PrimV  : Op -> W
+  | PairV  : W -> W -> W
+  | LamV   : forall {n}, VectorDef.t W n -> Exp (S n) -> W   (* closure *)
+.
+
+(* equality of domain values is decidable. *)
+Fixpoint W_eqb (v1 : W) (v2 : W) : bool := 
+  match v1 , v2 with 
+  | IntV k1 , IntV k2 => Nat.eqb k1 k2
+  | PairV v1 v2, PairV w1 w2 => W_eqb v1 w1 && W_eqb v2 w2
+  | PrimV o1 , PrimV o2 => Op_eqb o1 o2
+  | LamV _ _ , LamV _ _ => false  (* TODO *)
+  | _ , _ => false
+  end.
+
+Fixpoint W_size (v : W) : nat  := 
+  match v with 
+  | IntV k => k
+  | PairV v1 v2 => 1 + max (W_size v1) (W_size v2)
+  | PrimV o => 1
+  | LamV _ _ => 0  (* TODO *)
+  end.                                 
+
+Definition isLamV (v : W) := 
+  match v with 
+  | LamV _ _ => true
+  | _ => false
+  end.
+
+(* domain values can be effectively enumerated *)
+(* TODO: this excludes closures.... *)
+Fixpoint W_enum (n : nat) : list W := 
+  match n with 
+  | 0 => [IntV 0 ; PrimV op_Add ; PrimV op_Gt ; PrimV op_Int ]
+  | S n => let prev := W_enum n in 
+          prev ++ [IntV (S n)]
+               ++ List.flat_map (fun v1 => List.flat_map 
+                                          (fun v2 => [PairV v1 v2]%list) prev) prev
+  end.
+
+
+(* every (non-lambda) value is contained in the enumeration. *)
+Lemma enum_all : forall (v : W), (isLamV v) = false -> 
+                                      exists k, List.In v (W_enum k).
+Proof.
+  induction v.
+  all: intro h; simpl in h.
+  exists n. clear h. destruct n. simpl; auto. simpl; auto. admit.
+Admitted. 
+
+(* Enumerating more values extends the list. *)
+Lemma enum_mono : forall j k, j <= k -> (exists l, W_enum k = (W_enum j) ++ l)%list.
+Proof.
+  intros. induction H. exists nil. rewrite List.app_nil_r. auto.
+  move: IHle => [l E]. simpl.
+  eexists.
+  rewrite E.
+  rewrite <- List.app_assoc. 
+  eauto.
+Qed.
+
+End W.
+
+Section Monad.
+Import SetNotations.
+
+Definition M (A : Type) := P A.  (* set of values of type A *)
+
+Definition WRONG {A} : M A := ∅.
+Definition EMPTY {A} : M A := ∅.
+Definition UNIT  {A} : A -> M A := fun x => ⌈ x ⌉.
+Definition UNION {A} : M A -> M A -> M A := Union. 
+Definition INTER {A} : M A -> M A -> M A := Intersection.
+
+Definition SEQ {A} : M A -> M A -> M A := 
+  fun s1 s2 => (fun x => (exists y, s1 y) /\ s2 x).
+
+(* NOTE: if the semantics depends on there only being a unique value in the 
+   set, then it is *not* monotonic. Running evalExp with a larger n could
+   turn a singleton set into a non-singleton set.
+*)
+Definition ONE {A} : M A -> M A := 
+  fun s => (fun y => s ≃ ⌈ y ⌉).
+
+(* Note: since we only have binary pairs, this is a bit odd. ALL works when
+   there are two values in the set. However, having n-tuples would also
+   produce a non-monotonic operator. As the number of potential results grows,
+   then the size of the tuple *also* grows. This is not ideal.
+*)
+Definition ALL : M W -> M W := 
+  fun s => (fun y => match y with 
+                       | PairV w1 w2 => s w1 /\ s w2
+                       | _ => False
+                       end).
+
+(* Merge togther the result of the function f applied to every w in W (up to k) *)
+Definition ITERATE (k : nat) (f : W -> M W) : M W := 
+  unions (List.map f (W_enum k)).
+
+(* If we iterate more, then we only get larger results. *)
+Lemma ITERATE_mono : forall j k f, j <= k -> ITERATE j f ⊆ ITERATE k f.
+Proof.
+  intros. unfold ITERATE.
+  move: (enum_mono H) => [l h].
+  rewrite h.
+  eapply unions_enum_mono.
+Qed.
+
+End Monad.
+
+
+Section Semantics.
+
+Definition Env (n : nat) := VectorDef.t W n.
+Definition lookupEnv {n} (e : Env n) (x : Fin.t n) : W := VectorDef.nth e x. 
+
+(* semantics of values *)
+Fixpoint evalVal {n} (env : Env n) (V : Val n) : W :=
+  match V with 
+  | Var v => lookupEnv env v
+  | Lam e => LamV env e
+  | Pair v1 v2 => PairV (evalVal env v1) (evalVal env v2)
+  | Int k => IntV k
+  | Prim o => PrimV o
+  end.
+ 
+Definition evalPrim (o : Op) (w : W) : M W := 
+  match o , w with 
+  (* addition *)
+  | op_Add , PairV (IntV j) (IntV k) => UNIT (IntV (j+k))
+  | op_Add , _ => WRONG
+  (* Gt *)
+  | op_Gt  , PairV (IntV j) (IntV k) => 
+      if Nat.leb k j then UNIT ( IntV j ) else EMPTY
+  | op_Gt , _ => WRONG
+  (* type test: identity function on Int, fails when given a non int value *)
+  | op_Int , IntV k => UNIT ( IntV k )
+  | op_Int , _ => EMPTY
+  end.
+
+Import VectorDef.VectorNotations.
+
+(* semantics of expressions *)
+
+Fixpoint evalExp (m:nat) {n : nat} (env: Env n) (e: Exp n) : M W :=  
+  match m with 
+  | 0 => EMPTY
+  | S m' => match e with 
+           | Ret v => 
+               UNIT (evalVal env v)
+
+           | Fail_ => EMPTY
+
+           | Or e1 e2 => UNION (evalExp m' env e1) (evalExp m' env e2)
+
+           | Unify e1 e2 => INTER (evalExp m' env e1) (evalExp m' env e2)
+
+           | Seq e1 e2 => SEQ (evalExp m' env e1) (evalExp m' env e2)
+
+           | App e v => 
+               let w := evalVal env v in
+               match evalVal env e with                      
+                 | (LamV env1 e1) => evalExp m' (VectorDef.cons _ w _ env1) e1
+                 | PrimV p => evalPrim p w
+                 | _ => WRONG   (* non-function application *)
+               end
+
+           | Exists e => 
+               ITERATE m' (fun w => evalExp m' (VectorDef.cons _ w _ env) e)
+
+           | One e => ONE (evalExp m' env e)
+
+           | All e => ALL (evalExp m' env e)
+           end
+  end.
+
+End Semantics.
+
+(* Examples *)
+
+(* exists x. x = 3 ; x *)
+Definition ex : Exp 0 := 
+  Exists (Seq (Unify (Ret (Var F1)) (Ret (Int 3))) (Ret (Var F1))).
+
+Lemma evex : exists n, UNIT (IntV 3) ⊆ evalExp n (@VectorDef.nil _) ex.
+move: (enum_all (IntV 3) ltac:(reflexivity)) => [k h].
+exists (S (S (S (S k)))). 
+simpl.
+unfold ITERATE.
+remember (fun w : W => SEQ (INTER (UNIT w) (UNIT (IntV 3))) (UNIT w)) as f.
+apply List.in_map with (f:=f) in h.
+move: (unions_In _ _ h) => h1.
+have LT: k <= 3+k. econstructor; eauto. apply enum_mono in LT.
+move: LT => [l E]. rewrite E.
+rewrite <- unions_enum_mono.
+rewrite <- h1.
+rewrite Heqf. 
+intros x xIn. inversion xIn.
+cbv. split. exists (IntV 3). 
+constructor. auto. auto. constructor.
+Qed.
+
+(* exists x. x = 3 | x = 4 *)
+
+Definition ex : Exp 0 := 
+ Exists (Or (Unify (Ret (Var F1)) (Ret (Int 3)))
+            (Unify (Ret (Var F1)) (Ret (Int 4)))).
+
+Lemma evex : exists n, exists s,  evalExp n [] ex = Some s /\ s (IntV 3) /\ s (IntV 4).
+eexists.
+eexists.
+
+exists (⌈IntV 3⌉ ∪ ⌈IntV 4⌉).
+simpl. unfold ITERATE.
+
+(* exists x. x *)
+
