coq/verse/densem_pointed2.v
@@ -1,0 +1,257 @@
+Require Import Coq.Vectors.Fin.
+Require Coq.Vectors.VectorDef.
+Require List.
+Import List.ListNotations.
+
+Require Export ssreflect.
+Require Export Coq.Classes.RelationClasses.
+Require Import structures.Sets.
+Require structures.Option.
+
+(* This file defines a "denotational" semantics for Verse
+
+   M A := P (option A)
+
+   In this version, the denotation of an expression is a set of lifted values.
+
+   If the set is empty, the expression fails
+
+   What is Bottom? Not sure which is the appropriate answer
+     - the singleton set None?
+     - a set that contains None?
+
+   Allowing sets to contain both None and Some seems like it will be important 
+   to eventually supporting "one"
+
+   
+*)
+
+
+Set Implicit Arguments.
+
+Inductive Op : Type := op_Add | op_Gt | op_Int.
+
+Inductive Val (n: nat) : Type := 
+  | Var   : Fin.t n -> Val n
+  | Int   : nat -> Val n
+  | Prim  : Op -> Val n
+  | Pair  : Val n -> Val n -> Val n   (* todo: generalize to n-tuples *)
+  | Lam   : Exp (S n) -> Val n
+
+with Exp (n : nat): Type :=
+  | Ret    : Val n -> Exp n
+  | App    : Val n -> Val n -> Exp n  
+  | Seq    : Exp n -> Exp n -> Exp n
+
+  | Unify  : Exp n -> Exp n -> Exp n   
+  | Exists : Exp (S n) -> Exp n
+  | Or     : Exp n -> Exp n -> Exp n 
+  | Fail_  : Exp n
+  | One    : Exp n -> Exp n 
+  | All    : Exp n -> Exp n  
+.
+
+Arguments Int {_}.
+Arguments Prim {_}.
+Arguments Fail_ {_}.
+
+(* This is our domain of values (W): numbers, primitives, pairs of values 
+   and closures *)
+Inductive W : Type := 
+  | IntV   : nat -> W
+  | PrimV  : Op -> W
+  | PairV  : W -> W -> W
+  | LamV   : forall {n}, VectorDef.t W n -> Exp (S n) -> W   (* closure *)
+.
+
+Import SetNotations.
+
+
+Section Monad.
+
+Definition M (A : Type) := P (option A). 
+
+Definition BOTTOM {A} : M A := ⌈ None ⌉.
+Definition WRONG {A} : M A := ∅.
+Definition FAIL {A} : M A := ∅.
+Definition UNIT  {A} : A -> M A := fun x => ⌈ Some x ⌉.
+Definition UNION {A} : M A -> M A -> M A := Union.
+Definition INTER {A} : M A -> M A -> M A := Intersection.
+
+Definition SEQ {A} : M A -> M A -> M A := 
+  fun s1 s2 => 
+    fun x => 
+      match x with 
+      | None => (None ∈ s1) \/ (None ∈ s2)
+      | Some y => (exists z, Some z ∈ s1) /\ not (None ∈ s1) /\ (Some y ∈ s2)
+      end.
+
+(* This is still not correct because we cannot pick an element. *)
+Definition ONE {A} : M A -> M A := 
+  (fun s => s).
+
+(* Note: WEIRD semantics. All pairs of elements in the interpretation. Not 
+  a singleton. *)
+Definition ALL : M W -> M W := 
+  (fun s => (fun y => match y with 
+                       | None => None ∈ s
+                       | Some (PairV w1 w2) => s (Some w1) /\ s (Some w2)
+                       | _ => False
+                       end)).
+
+(* Merge togther the result of the function f applied to every w in W. *)
+(* - only diverges if *all* f w diverge
+   - contains all elements produced by some f w
+   - ff all f w fail, then fails
+ *)
+Definition EXISTS {A} (f : A -> M A) : M A := 
+ (fun x => match x with 
+          | None => forall w, ⌈ None ⌉ ≃ (f w)
+          | Some y => exists w, Some y ∈ f w
+        end).
+
+(* Maybe do something special for functions??? *)
+Definition EQUAL {A} : M A -> M A -> Prop := fun x y => x ≃ y.
+
+End Monad.
+
+
+Section Semantics.
+
+Definition Env (n : nat) := VectorDef.t W n.
+Definition lookupEnv {n} (e : Env n) (x : Fin.t n) : W := VectorDef.nth e x. 
+
+(* semantics of values *)
+Fixpoint evalVal {n} (env : Env n) (V : Val n) : W :=
+  match V with 
+  | Var v => lookupEnv env v
+  | Lam e => LamV env e
+  | Pair v1 v2 => PairV (evalVal env v1) (evalVal env v2)
+  | Int k => IntV k
+  | Prim o => PrimV o
+  end.
+ 
+Definition evalPrim (o : Op) (w : W) : M W := 
+  match o , w with 
+  (* addition *)
+  | op_Add , PairV (IntV j) (IntV k) => UNIT (IntV (j+k))
+  | op_Add , _ => WRONG
+  (* Gt *)
+  | op_Gt  , PairV (IntV j) (IntV k) => 
+      if Nat.leb k j then UNIT ( IntV j ) else FAIL
+  | op_Gt , _ => WRONG
+  (* type test: identity function on Int, fails when given a non int value *)
+  | op_Int , IntV k => UNIT ( IntV k )
+  | op_Int , _ => FAIL
+  end.
+
+Import VectorDef.VectorNotations.
+
+(* semantics of expressions *)
+
+Fixpoint evalExp (m:nat) {n : nat} (env: Env n) (e: Exp n) : M W :=  
+  match m with 
+  | 0 => BOTTOM
+  | S m' => match e with 
+           | Ret v => 
+               UNIT (evalVal env v)
+
+           | Fail_ => FAIL
+
+           | Or e1 e2 => UNION (evalExp m' env e1) (evalExp m' env e2)
+
+           | Unify e1 e2 => INTER (evalExp m' env e1) (evalExp m' env e2)
+
+           | Seq e1 e2 => SEQ (evalExp m' env e1) (evalExp m' env e2)
+
+           | App e v => 
+               let w := evalVal env v in
+               match evalVal env e with                      
+                 | (LamV env1 e1) => evalExp m' (VectorDef.cons _ w _ env1) e1
+                 | PrimV p => evalPrim p w
+                 | _ => WRONG   (* non-function application *)
+               end
+
+           | Exists e => 
+               EXISTS (fun w => evalExp m' (VectorDef.cons _ w _ env) e)
+
+           | One e => ONE (evalExp m' env e)
+
+           | All e => ALL (evalExp m' env e)
+           end
+  end.
+
+End Semantics.
+
+
+Import VectorDef.VectorNotations.
+
+(* Examples *)
+
+(* exists x. x = 3 ; x *)
+Definition ex0 : Exp 0 := 
+  Exists (Seq (Unify (Ret (Var F1)) (Ret (Int 3))) (Ret (Var F1))).
+
+Lemma evex0 : exists n, EQUAL (UNIT (IntV 3)) (evalExp n (@VectorDef.nil _) ex0).
+exists 4. 
+simpl.
+split.
+- unfold EXISTS.
+  intros x xIn. inversion xIn.
+  exists (IntV 3). 
+  split.
+  exists (IntV 3).
+  repeat econstructor; eauto.
+  repeat econstructor; eauto.
+- unfold EXISTS.
+  intros x xIn. inversion xIn.
+  cbv in H.
+  move: H => [[y h1] h2].  inversion h2. subst.
+  inversion h1. subst. inversion H. subst. inversion H0. subst.
+  auto.
+Qed.
+
+(* exists x. x = 3 | x = 4 *)
+
+Definition ex1 : Exp 0 := 
+ Exists (Or (Unify (Ret (Var F1)) (Ret (Int 3)))
+            (Unify (Ret (Var F1)) (Ret (Int 4)))).
+
+Lemma evex1 : exists n, EQUAL (evalExp n (@VectorDef.nil _) ex1) 
+                     (UNION (UNIT (IntV 3)) (UNIT (IntV 4))).
+exists 10.
+simpl.
+unfold EXISTS.
+split.
+- intros x xIn. inversion xIn. clear xIn.
+  inversion H. subst.
+  inversion H0. subst.
+  inversion H1. inversion H2. subst.
+  left. auto.
+  inversion H0. inversion H2. inversion H3. subst.
+  right. auto.
+- intros x xIn. inversion xIn; subst; clear xIn; inversion H; clear H.
+  + exists (IntV 3).
+    constructor. constructor. auto. auto.
+  + exists (IntV 4).
+    right. constructor. auto. auto.
+Qed.
+
+(* 
+    exists x. x 1 = 2 ; x 1 
+*)
+
+Definition ex2 : Exp 0 := 
+  Exists (Seq (Unify (App (Var F1) (Int 1)) (Ret (Int 2)))
+              (App (Var F1) (Int 1))).
+
+(* We can show that "2" is in the meaning of this expression *)
+Lemma evex2 : exists n, IntV 2 ∈ evalExp n (@VectorDef.nil _) ex2.
+Proof.
+  exists 5.
+  exists (LamV (@VectorDef.nil _) (Ret (Int 2))).
+  cbv.
+  split; eauto. exists (IntV 2). constructor; eauto. constructor; eauto.
+Qed.
+
+(* if (x=1) then (2 3) else 4; x=(1 2); if (x=1) then 5 else (6 7) *)
